@prefix : <http://www.qualityreport.com/qr/>.
@prefix dcat:<http://www.w3.org/ns/dcat#>. 
@prefix dcterms:<http://purl.org/dc/terms/>.
@prefix xsd:<http://www.w3.org/2001/XMLSchema#>.
@prefix dqv:<http://www.w3.org/ns/dqv#>.
@prefix skos:<http://www.w3.org/2004/02/skos/core#>.
@prefix ldqd:<http://www.w3.org/2016/05/ldqd#> .
@prefix dct:<http://purl.org/dc/terms/>.
@prefix qb:<http://purl.org/linked-data/cube#>.
@prefix owl:<http://www.w3.org/2002/07/owl#>.
@prefix rdf:<http://www.w3.org/1999/02/22-rdf-syntax-ns#>.
@prefix rdfs:<http://www.w3.org/2000/01/rdf-schema#>.

#################################################################################
#### Quality Report  ###
#################################################################################

:myCatalog a dcat:Catalog ;
    dcterms:title "datos.gob.es catalog";
    dqv:hasQualityMeasurement 
    	:DQCompletenessCommission_dataset_automatic,
    	:DQCompletenessCommission_distribution_automatic,
		:DQCompletenessOmission_dataset_automatic,
		:DQCompletenessOmission_distribution_automatic, 
		:DQConceptualConsistency_dataset_automatic, 
		:DQConceptualConsistency_distribution_automatic, 
		:DQConceptualConsistency_distribution_format_accessURL_automatic, 
		:DQDomainConsistency_dataset_title_automatic,
		:DQDomainConsistency_dataset_description_automatic, 
		:DQDomainConsistency_dataset_theme_automatic, 
		:DQDomainConsistency_dataset_keyword_automatic, 
		:DQDomainConsistency_dataset_identifier_automatic,
		:DQDomainConsistency_dataset_issued_automatic, 
		:DQDomainConsistency_dataset_modified_automatic,
		:DQDomainConsistency_dataset_accrualPeriodicity_automatic, 
		:DQDomainConsistency_dataset_language_automatic, 
		:DQDomainConsistency_dataset_publisher_automatic, 
		:DQDomainConsistency_dataset_spatial_automatic, 
		:DQDomainConsistency_dataset_temporal_automatic, 
		:DQDomainConsistency_dataset_valid_automatic, 
		:DQDomainConsistency_dataset_references_automatic,
		:DQDomainConsistency_dataset_conformsTo_automatic,
		:DQDomainConsistency_dataset_distribution_automatic,
		:DQDomainConsistency_distribution_identifier_automatic, 
		:DQDomainConsistency_distribution_title_automatic, 
		:DQDomainConsistency_distribution_accessURL_automatic, 
		:DQDomainConsistency_distribution_format_automatic, 
		:DQDomainConsistency_distribution_byteSize_automatic, 
		:DQDomainConsistency_distribution_license_automatic, 
		:DQTemporalConsistency_dataset_issued_modified_valid_automatic, 
		:DQTemporalValidity_dataset_issued_modified_valid_automatic, 
		:DQThematicClassificationCorrectness_dataset_theme_manual, 
		:DQNonQuantitativeAttributeCorrectness_dataset_references_manual,
		:DQNonQuantitativeAttributeCorrectness_dataset_conformsTo_manual,
		:DQNonQuantitativeAttributeCorrectness_dataset_accessURL_manual,
		:DQNonQuantitativeAttributeCorrectness_dataset_license_manual,
		:DQNonQuantitativeAttributeCorrectness_distribution_references_automatic,
		:DQNonQuantitativeAttributeCorrectness_distribution_conformsTo_automatic,
		:DQNonQuantitativeAttributeCorrectness_distribution_accessURL_automatic,
		:DQNonQuantitativeAttributeCorrectness_distribution_license_automatic,
		:DQPositionalCorrectness_dataset_spatial_automatic, 
		:DQQualityOfFreeText_dataset_title_manual,
		:DQQualityOfFreeText_dataset_description_manual,
		:DQQualityOfFreeText_dataset_title_automatic,
		:DQQualityOfFreeText_dataset_description_automatic.

#################################################################################
#### Completeness  ###

:DQCompleteness a dqv:Dimension ;
	dqv:inCategory ldqd:intrinsicDimensions ;
    skos:prefLabel "DQ_Completeness"@en;
    skos:definition "Presence or absence of metadata elements."@en .

#--------------------------------------

:DQCompletenessCommission skos:broader :DQCompleteness;
    skos:prefLabel "DQ_CompletenessCommission"@en;
    skos:definition "Checking for excess instances of metadata elements in a metadata record."@en .

:D.3.ISO.19157 a dqv:Metric ;
    skos:definition "Rate of records with excess items."@en ;
    dqv:inDimension :DQCompletenessCommission;
    dqv:expectedDataType xsd:boolean.

:DQCompletenessCommission_dataset_automatic a dqv:QualityMeasurement ;
    dqv:computedOn :myCatalog ;
    dqv:isMeasurementOf :D.3.ISO.19157 ;
    dqv:value "true"^^xsd:boolean;
    dct:date "2020-03-01"^^xsd:date ;
    :onProperty dcat:dataset.

:DQCompletenessCommission_distribution_automatic a dqv:QualityMeasurement ;
    dqv:computedOn :myCatalog ;
    dqv:isMeasurementOf :D.3.ISO.19157 ;
    dqv:value "true"^^xsd:boolean;
    dct:date "2020-03-01"^^xsd:date ;
    :onProperty dcat:distribution. 

#--------------------------------------

:DQCompletenessOmission skos:broader :DQCompleteness;
    skos:prefLabel "DQ_CompletenessOmmission"@en;
    skos:definition "Checking for mandatory elements that are absent in metadata records."@en .

:D.7.ISO.19157 a dqv:Metric ;
    skos:definition "Rate of records with missing items."@en ;
    dqv:inDimension :DQCompletenessOmission;
    dqv:expectedDataType xsd:boolean.

:DQCompletenessOmission_dataset_automatic a dqv:QualityMeasurement ;
    dqv:computedOn :myCatalog ;
    dqv:isMeasurementOf :D.7.ISO.19157 ;
    dqv:value "true"^^xsd:boolean;
    dct:date "2020-03-01"^^xsd:date ;
    :onProperty dcat:dataset.

:DQCompletenessOmission_distribution_automatic a dqv:QualityMeasurement ;
    dqv:computedOn :myCatalog ;
    dqv:isMeasurementOf :D.7.ISO.19157 ;
    dqv:value "false"^^xsd:boolean;
    dct:date "2020-03-01"^^xsd:date ;
    :onProperty dcat:distribution.

##################################################################################
### Logical Consistency

:DQLogicalConsistency a dqv:Dimension ;
	dqv:inCategory ldqd:intrinsicDimensions ;
    skos:prefLabel "DQ_LogicalConsistency"@en;
    skos:definition "Determining the degree of adherence to logical rules of metadata structure."@en. 

#--------------------------------------

:DQConceptualConsistency skos:broader :DQLogicalConsistency;
    skos:prefLabel "DQ_ConceptualConsistency"@en;
    skos:definition "Determining the adherence to the metadata schema or to other explicit or non-explicit requirements of a data model or a dataset."@en .

:D.13.ISO.19157 a dqv:Metric ;
    skos:definition "Rate of records compliant with the conceptual schema."@en ;
    dqv:inDimension :DQConceptualConsistency;
    dqv:expectedDataType xsd:boolean.

:DQConceptualConsistency_dataset_automatic a dqv:QualityMeasurement ;
    dqv:computedOn :myCatalog ;
    dqv:isMeasurementOf :D.13.ISO.19157 ;
    dqv:value "true"^^xsd:boolean;
    dct:date "2020-03-01"^^xsd:date ;
    :onProperty dcat:dataset.

:DQConceptualConsistency_distribution_automatic a dqv:QualityMeasurement ;
    dqv:computedOn :myCatalog ;
    dqv:isMeasurementOf :D.13.ISO.19157 ;
    dqv:value "false"^^xsd:boolean;
    dct:date "2020-03-01"^^xsd:date ;
    :onProperty dcat:distribution.

:DQConceptualConsistency_distribution_format_accessURL_automatic a dqv:QualityMeasurement ;
    dqv:computedOn :myCatalog ;
    dqv:isMeasurementOf :D.13.ISO.19157 ;
    dqv:value "false"^^xsd:boolean;
    dct:date "2020-03-01"^^xsd:date ;
    :onProperty dcat:distribution, dct:format, dcat:accessURL.

#:SimD.22.ISO.19157 a dqv:Metric ;
#    skos:definition "Number of records with inconsistent information in metadata elements."@en ;
#    dqv:inDimension :DQConceptualConsistency;
#    dqv:expectedDataType xsd:boolean.

#--------------------------------------

:DQDomainConsistency skos:broader :DQLogicalConsistency;
    skos:prefLabel "DQ_DomainConsistency"@en;
    skos:definition "Determining the adherence of metadata element values to the value domains."@en .

:D.17.ISO.19157 a dqv:Metric ;
    skos:definition "Value domain conformance rate."@en ;
    dqv:inDimension :DQDomainConsistency;
    dqv:expectedDataType xsd:boolean.

:DQDomainConsistency_dataset_title_automatic a dqv:QualityMeasurement ;
    dqv:computedOn :myCatalog ;
    dqv:isMeasurementOf :D.17.ISO.19157 ;
    dqv:value "true"^^xsd:boolean;
    dct:date "2020-03-01"^^xsd:date ;
    :onProperty dcat:dataset, dct:title.

:DQDomainConsistency_dataset_description_automatic a dqv:QualityMeasurement ;
    dqv:computedOn :myCatalog ;
    dqv:isMeasurementOf :D.17.ISO.19157 ;
    dqv:value "true"^^xsd:boolean;
    dct:date "2020-03-01"^^xsd:date ;
    :onProperty dcat:dataset, dct:description.

:DQDomainConsistency_dataset_theme_automatic a dqv:QualityMeasurement ;
    dqv:computedOn :myCatalog ;
    dqv:isMeasurementOf :D.17.ISO.19157 ;
    dqv:value "true"^^xsd:boolean;
    dct:date "2020-03-01"^^xsd:date ;
    :onProperty dcat:dataset, dcat:theme.

:DQDomainConsistency_dataset_keyword_automatic a dqv:QualityMeasurement ;
    dqv:computedOn :myCatalog ;
    dqv:isMeasurementOf :D.17.ISO.19157 ;
    dqv:value "true"^^xsd:boolean;
    dct:date "2020-03-01"^^xsd:date ;
    :onProperty dcat:dataset, dcat:keyword.

:DQDomainConsistency_dataset_identifier_automatic a dqv:QualityMeasurement ;
    dqv:computedOn :myCatalog ;
    dqv:isMeasurementOf :D.17.ISO.19157 ;
    dqv:value "false"^^xsd:boolean;
    dct:date "2020-03-01"^^xsd:date ;
    :onProperty dcat:dataset, dct:identifier.

:DQDomainConsistency_dataset_issued_automatic a dqv:QualityMeasurement ;
    dqv:computedOn :myCatalog ;
    dqv:isMeasurementOf :D.17.ISO.19157 ;
    dqv:value "true"^^xsd:boolean;
    dct:date "2020-03-01"^^xsd:date ;
    :onProperty dcat:dataset, dct:issued.

:DQDomainConsistency_dataset_modified_automatic a dqv:QualityMeasurement ;
    dqv:computedOn :myCatalog ;
    dqv:isMeasurementOf :D.17.ISO.19157 ;
    dqv:value "true"^^xsd:boolean;
    dct:date "2020-03-01"^^xsd:date ;
    :onProperty dcat:dataset, dct:modified.

:DQDomainConsistency_dataset_accrualPeriodicity_automatic a dqv:QualityMeasurement ;
    dqv:computedOn :myCatalog ;
    dqv:isMeasurementOf :D.17.ISO.19157 ;
    dqv:value "true"^^xsd:boolean;
    dct:date "2020-03-01"^^xsd:date ;
    :onProperty dcat:dataset, dct:accrualPeriodicity.

:DQDomainConsistency_dataset_language_automatic a dqv:QualityMeasurement ;
    dqv:computedOn :myCatalog ;
    dqv:isMeasurementOf :D.17.ISO.19157 ;
    dqv:value "true"^^xsd:boolean;
    dct:date "2020-03-01"^^xsd:date ;
    :onProperty dcat:dataset, dct:language.

:DQDomainConsistency_dataset_publisher_automatic a dqv:QualityMeasurement ;
    dqv:computedOn :myCatalog ;
    dqv:isMeasurementOf :D.17.ISO.19157 ;
    dqv:value "true"^^xsd:boolean;
    dct:date "2020-03-01"^^xsd:date ;
    :onProperty dcat:dataset, dct:publisher.

:DQDomainConsistency_dataset_spatial_automatic a dqv:QualityMeasurement ;
    dqv:computedOn :myCatalog ;
    dqv:isMeasurementOf :D.17.ISO.19157 ;
    dqv:value "false"^^xsd:boolean;
    dct:date "2020-03-01"^^xsd:date ;
    :onProperty dcat:dataset, dct:spatial.

:DQDomainConsistency_dataset_temporal_automatic a dqv:QualityMeasurement ;
    dqv:computedOn :myCatalog ;
    dqv:isMeasurementOf :D.17.ISO.19157 ;
    dqv:value "true"^^xsd:boolean;
    dct:date "2020-03-01"^^xsd:date ;
    :onProperty dcat:dataset, dct:temporal.

:DQDomainConsistency_dataset_valid_automatic a dqv:QualityMeasurement ;
    dqv:computedOn :myCatalog ;
    dqv:isMeasurementOf :D.17.ISO.19157 ;
    dqv:value "true"^^xsd:boolean;
    dct:date "2020-03-01"^^xsd:date ;
    :onProperty dcat:dataset, dct:valid.

:DQDomainConsistency_dataset_references_automatic a dqv:QualityMeasurement ;
    dqv:computedOn :myCatalog ;
    dqv:isMeasurementOf :D.17.ISO.19157 ;
    dqv:value "true"^^xsd:boolean;
    dct:date "2020-03-01"^^xsd:date ;
    :onProperty dcat:dataset, dct:references.

:DQDomainConsistency_dataset_conformsTo_automatic a dqv:QualityMeasurement ;
    dqv:computedOn :myCatalog ;
    dqv:isMeasurementOf :D.17.ISO.19157 ;
    dqv:value "true"^^xsd:boolean;
    dct:date "2020-03-01"^^xsd:date ;
    :onProperty dcat:dataset, dct:conformsTo.

:DQDomainConsistency_dataset_distribution_automatic a dqv:QualityMeasurement ;
    dqv:computedOn :myCatalog ;
    dqv:isMeasurementOf :D.17.ISO.19157 ;
    dqv:value "true"^^xsd:boolean;
    dct:date "2020-03-01"^^xsd:date ;
    :onProperty dcat:distribution.

:DQDomainConsistency_distribution_identifier_automatic a dqv:QualityMeasurement ;
    dqv:computedOn :myCatalog ;
    dqv:isMeasurementOf :D.17.ISO.19157 ;
    dqv:value "true"^^xsd:boolean;
    dct:date "2020-03-01"^^xsd:date ;
    :onProperty dcat:distribution,dct:identifier.

:DQDomainConsistency_distribution_title_automatic a dqv:QualityMeasurement ;
    dqv:computedOn :myCatalog ;
    dqv:isMeasurementOf :D.17.ISO.19157 ;
    dqv:value "true"^^xsd:boolean;
    dct:date "2020-03-01"^^xsd:date ;
    :onProperty dcat:distribution,dct:title.

:DQDomainConsistency_distribution_accessURL_automatic a dqv:QualityMeasurement ;
    dqv:computedOn :myCatalog ;
    dqv:isMeasurementOf :D.17.ISO.19157 ;
    dqv:value "true"^^xsd:boolean;
    dct:date "2020-03-01"^^xsd:date ;
    :onProperty dcat:distribution,dcat:accessURL.

:DQDomainConsistency_distribution_format_automatic a dqv:QualityMeasurement ;
    dqv:computedOn :myCatalog ;
    dqv:isMeasurementOf :D.17.ISO.19157 ;
    dqv:value "false"^^xsd:boolean;
    dct:date "2020-03-01"^^xsd:date ;
    :onProperty dcat:distribution,dct:format.

:DQDomainConsistency_distribution_byteSize_automatic a dqv:QualityMeasurement ;
    dqv:computedOn :myCatalog ;
    dqv:isMeasurementOf :D.17.ISO.19157 ;
    dqv:value "true"^^xsd:boolean;
    dct:date "2020-03-01"^^xsd:date ;
    :onProperty dcat:distribution,dcat:byteSize.

:DQDomainConsistency_distribution_license_automatic a dqv:QualityMeasurement ;
    dqv:computedOn :myCatalog ;
    dqv:isMeasurementOf :D.17.ISO.19157 ;
    dqv:value "true"^^xsd:boolean;
    dct:date "2020-03-01"^^xsd:date ;
    :onProperty dcat:distribution,dct:license.

#--------------------------------------

#:DQFormatConsistency skos:broader :DQLogicalConsistency;
#    skos:prefLabel "DQ_FormatConsistency"@en;
#    skos:definition "Verifying the use of the appropriate format for metadata encoding."@en.

#:D21.ISO.19157 a dqv:Metric ;
#    skos:definition "Physical structure conflict rate."@en ;
#    dqv:inDimension :DQFormatConsistency;
#    dqv:expectedDataType xsd:boolean.

#--------------------------------------

#:DQTopologicalConsistency skos:broader :DQLogicalConsistency;
#    skos:prefLabel "DQ_TopologicalConsistency"@en;
#    skos:definition "Determining the correctness of the way in which constituent parts are interrelated or arranged in terms of metadata."@en .

#:D23.ISO.19157 a dqv:Metric ;
#    skos:definition "Rate of records having faulty relationships with other records in the catalogue."@en ;
#    dqv:inDimension :DQTopologicalConsistency;
#    dqv:expectedDataType xsd:boolean.

#:TopologicalContradiction a dqv:Metric ;
#    skos:definition "Rate of records having faulty relationships between two metadata elements of the same record."@en ;
#    dqv:inDimension :DQTopologicalConsistency;
#    dqv:expectedDataType xsd:boolean.

##################################################################################
### Temporal Accuracy

:DQTemporalQuality a dqv:Dimension ;
	dqv:inCategory ldqd:intrinsicDimensions ;
    skos:prefLabel "DQ_TemporalQuality"@en;
    skos:definition "Determining the accuracy of the temporal metadata elements and temporal relationships of metadata elements."@en .
 
#--------------------------------------

:DQTemporalConsistency skos:broader :DQDQTemporalQuality;
    skos:prefLabel "DQ_TemporalConsistency"@en;
    skos:definition "Determining the correctness of ordered events or sequences, if reported, within a single metadata record."@en.

:SimD26.ISO.19157S a dqv:Metric ;
    skos:definition "Rate of records with conflict time sequences."@en;
    dqv:inDimension :DQTemporalConsistency;
    dqv:expectedDataType xsd:boolean.

:DQTemporalConsistency_dataset_issued_modified_valid_automatic a dqv:QualityMeasurement ;
    dqv:computedOn :myCatalog ;
    dqv:isMeasurementOf :SimD26.ISO.19157S ;
    dqv:value "false"^^xsd:boolean;
    dct:date "2020-03-01"^^xsd:date ;
    :onProperty dcat:dataset, dct:issued, dct:modified, dct:valid.

#--------------------------------------

:DQTemporalValidity skos:broader :DQTemporalAccuracy;
    skos:prefLabel "DQ_TemporalValidity"@en;
    skos:definition "Determining the validity of metadata time values with respect to a defined time range."@en.

:D18.ISO.19157S a dqv:Metric ;
    skos:definition "Value domain non-conformance rate."@en;
    dqv:inDimension :DQTemporalValidity;
    dqv:expectedDataType xsd:boolean.

:DQTemporalValidity_dataset_issued_modified_valid_automatic a dqv:QualityMeasurement ;
    dqv:computedOn :myCatalog ;
    dqv:isMeasurementOf :D18.ISO.19157S ;
    dqv:value "true"^^xsd:boolean;
    dct:date "2020-03-01"^^xsd:date ;
    :onProperty dcat:dataset, dct:issued, dct:modified, dct:valid.

##################################################################################
### Thematic Accuracy

:DQThematicAccuracy a dqv:Dimension ;
	dqv:inCategory ldqd:intrinsicDimensions ;
    skos:prefLabel "DQ_ThematicAccuracy"@en;
    skos:definition "Determining the correctness of non-quantitative metadata elements and metadata elements related to classifications."@en .
 
#--------------------------------------

:DQThematicClassificationCorrectness skos:broader :DQThematicAccuracy;
    skos:prefLabel "DQ_ThematicClassificationCorrectness"@en;
    skos:definition "Determining the correctness of the thematic keywords and categories included in the metadata with respect to a universe of discourse."@en.

:D63.ISO.19157S a dqv:Metric ;
    skos:definition "Number of incorrectly classified records."@en;
    dqv:inDimension :DQThematicClassificationCorrectness;
    dqv:expectedDataType xsd:boolean.

:DQThematicClassificationCorrectness_dataset_theme_manual a dqv:QualityMeasurement ;
    dqv:computedOn :myCatalog ;
    dqv:isMeasurementOf :D63.ISO.19157S ;
    dqv:value "false"^^xsd:boolean;
    dct:date "2020-03-01"^^xsd:date ;
    :onProperty dcat:dataset, dcat:theme.

#--------------------------------------

:DQNonQuantitativeAttributeCorrectness skos:broader :DQThematicAccuracy;
    skos:prefLabel "DQ_NonQuantitativeAttributeCorrectness"@en;
    skos:definition "Determining the correctness of non-quantitative metadata elements in relation to a universe of discourse."@en.

:D68.ISO.19157S a dqv:Metric ;
    skos:definition "Number of incorrect attribute values."@en;
    dqv:inDimension :DQNonQuantitativeAttributeCorrectness;
    dqv:expectedDataType xsd:boolean.

:DQNonQuantitativeAttributeCorrectness_dataset_references_manual a dqv:QualityMeasurement ;
    dqv:computedOn :myCatalog ;
    dqv:isMeasurementOf :D68.ISO.19157S ;
    dqv:value "false"^^xsd:boolean;
    dct:date "2020-03-01"^^xsd:date ;
    :onProperty dcat:dataset, dct:references.

:DQNonQuantitativeAttributeCorrectness_dataset_conformsTo_manual a dqv:QualityMeasurement ;
    dqv:computedOn :myCatalog ;
    dqv:isMeasurementOf :D68.ISO.19157S ;
    dqv:value "false"^^xsd:boolean;
    dct:date "2020-03-01"^^xsd:date ;
    :onProperty dcat:dataset, dct:conformsTo.

:DQNonQuantitativeAttributeCorrectness_dataset_accessURL_manual a dqv:QualityMeasurement ;
    dqv:computedOn :myCatalog ;
    dqv:isMeasurementOf :D68.ISO.19157S ;
    dqv:value "true"^^xsd:boolean;
    dct:date "2020-03-01"^^xsd:date ;
    :onProperty dcat:dataset, dcat:accessURL.

:DQNonQuantitativeAttributeCorrectness_dataset_license_manual a dqv:QualityMeasurement ;
    dqv:computedOn :myCatalog ;
    dqv:isMeasurementOf :D68.ISO.19157S ;
    dqv:value "false"^^xsd:boolean;
    dct:date "2020-03-01"^^xsd:date ;
    :onProperty dcat:dataset, dct:license.

:D69.ISO.19157S a dqv:Metric ;
    skos:definition "Rate of incorrect attribute values."@en;
    dqv:inDimension :DQNonQuantitativeAttributeCorrectness;
    dqv:expectedDataType xsd:boolean.

:DQNonQuantitativeAttributeCorrectness_distribution_references_automatic a dqv:QualityMeasurement ;
    dqv:computedOn :myCatalog ;
    dqv:isMeasurementOf :D69.ISO.19157S ;
    dqv:value "false"^^xsd:boolean;
    dct:date "2020-03-01"^^xsd:date ;
    :onProperty dcat:distribution, dct:references.

:DQNonQuantitativeAttributeCorrectness_distribution_conformsTo_automatic a dqv:QualityMeasurement ;
    dqv:computedOn :myCatalog ;
    dqv:isMeasurementOf :D69.ISO.19157S ;
    dqv:value "false"^^xsd:boolean;
    dct:date "2020-03-01"^^xsd:date ;
    :onProperty dcat:distribution, dct:conformsTo.

:DQNonQuantitativeAttributeCorrectness_distribution_accessURL_automatic a dqv:QualityMeasurement ;
    dqv:computedOn :myCatalog ;
    dqv:isMeasurementOf :D69.ISO.19157S ;
    dqv:value "false"^^xsd:boolean;
    dct:date "2020-03-01"^^xsd:date ;
    :onProperty dcat:distribution, dcat:accessURL.

:DQNonQuantitativeAttributeCorrectness_distribution_license_automatic a dqv:QualityMeasurement ;
    dqv:computedOn :myCatalog ;
    dqv:isMeasurementOf :D69.ISO.19157S ;
    dqv:value "false"^^xsd:boolean;
    dct:date "2020-03-01"^^xsd:date ;
    :onProperty dcat:distribution, dct:license.


##################################################################################
### Positional Correctness

:DQPositionalCorrectness a dqv:Dimension ;
	dqv:inCategory ldqd:intrinsicDimensions ;
    skos:prefLabel "DQ_PositionalCorrectness"@en;
    skos:definition "As metadata often refers to locations (e.g.,the geographic extent of resources) but these locations are not spatial data
					themselves,  this  new  quality  element  was  proposed  to  check  correction rather than accuracy."@en .
 
:SimD33.ISO.19157S a dqv:Metric ;
    skos:definition "Rate of records with positional errors:  no overlap-ping between direct and indirect georeferences."@en;
    dqv:inDimension :DQPositionalCorrectness;
    dqv:expectedDataType xsd:boolean.

:DQPositionalCorrectness_dataset_spatial_automatic a dqv:QualityMeasurement ;
    dqv:computedOn :myCatalog ;
    dqv:isMeasurementOf :SimD33.ISO.19157S ;
    dqv:value "true"^^xsd:boolean;
    dct:date "2020-03-01"^^xsd:date ;
    :onProperty dcat:dataset, dct:spatial.

##################################################################################
### Quality of Free Text

:DQQualityOfFreeText a dqv:Dimension ;
	dqv:inCategory ldqd:intrinsicDimensions ;
    skos:prefLabel "DQ_QualityOfFreeText"@en;
    skos:definition "Because ISO 19157 had no adequate measures for descriptive and prosaic texts, this new quality element was proposed to evaluate the editorial content of free-text metadata elements."@en.

:OverallQualityOfFreeText a dqv:Metric ;
    skos:definition "Number of metadata element values with a bad quality level."@en;
    dqv:inDimension :DQQualityOfFreeText;
    dqv:expectedDataType xsd:boolean.

:DQQualityOfFreeText_dataset_title_manual a dqv:QualityMeasurement ;
    dqv:computedOn :myCatalog ;
    dqv:isMeasurementOf :OverallQualityOfFreeText ;
    dqv:value "false"^^xsd:boolean;
    dct:date "2020-03-01"^^xsd:date ;
    :onProperty dcat:dataset, dct:title;
    :onLanguage "es".

:DQQualityOfFreeText_dataset_description_manual a dqv:QualityMeasurement ;
    dqv:computedOn :myCatalog ;
    dqv:isMeasurementOf :OverallQualityOfFreeText ;
    dqv:value "true"^^xsd:boolean;
    dct:date "2020-03-01"^^xsd:date ;
    :onProperty dcat:dataset, dct:description;
    :onLanguage "es".

:ReadibilityOfTreeText a dqv:Metric ;
    skos:definition "Rate of metadata element values considered readable with a readability index (e.g. Flesch) above a threshold."@en;
    dqv:inDimension :DQQualityOfFreeText;
    dqv:expectedDataType xsd:boolean.

:DQQualityOfFreeText_dataset_title_automatic a dqv:QualityMeasurement ;
    dqv:computedOn :myCatalog ;
    dqv:isMeasurementOf :ReadibilityOfTreeText ;
    dqv:value "false"^^xsd:boolean;
    dct:date "2020-03-01"^^xsd:date ;
    :onProperty dcat:dataset, dct:title;
    :onLanguage "es".

:DQQualityOfFreeText_dataset_description_automatic a dqv:QualityMeasurement ;
    dqv:computedOn :myCatalog ;
    dqv:isMeasurementOf :ReadibilityOfTreeText ;
    dqv:value "false"^^xsd:boolean;
    dct:date "2020-03-01"^^xsd:date ;
    :onProperty dcat:dataset, dct:description;
    :onLanguage "es".

##################################################################################
### Extra properties in the model

#Parameters of the measurements (derived from DQV specification)
:onLanguage
    a qb:DimensionProperty, owl:DatatypeProperty ;
    rdfs:comment   "Language on which the quality measure is assessed."@en ;
    rdfs:domain    dqv:QualityMeasurement;
    rdfs:label     "Label assessment language"@en ;
    rdfs:range       xsd:string.

:onProperty
    a qb:DimensionProperty, rdf:Property ;
    rdfs:comment 	"Property on which the quality measure is assessed."@en ;
    rdfs:domain 	dqv:QualityMeasurement ;
    rdfs:label  	"Label assessment property"@en ;
    rdfs:range     	rdf:Property.

