@prefix : <http://www.qualityreport.com/qr/> .
@prefix dcat: <http://www.w3.org/ns/dcat#> .
@prefix dct: <http://purl.org/dc/terms/> .
@prefix dcterms: <http://purl.org/dc/terms/> .
@prefix dqv: <http://www.w3.org/ns/dqv#> .
@prefix ldqd: <http://www.w3.org/2016/05/ldqd#> .
@prefix owl: <http://www.w3.org/2002/07/owl#> .
@prefix prov: <http://www.w3.org/ns/prov#> .
@prefix qb: <http://purl.org/linked-data/cube#> .
@prefix rdf: <http://www.w3.org/1999/02/22-rdf-syntax-ns#> .
@prefix rdfs: <http://www.w3.org/2000/01/rdf-schema#> .
@prefix skos: <http://www.w3.org/2004/02/skos/core#> .
@prefix xml: <http://www.w3.org/XML/1998/namespace> .
@prefix xsd: <http://www.w3.org/2001/XMLSchema#> .

:D63.ISO.19157_conformance a dqv:Metric ;
    skos:definition "Checks if the number of incorrectly classified records is below Ac (maximum number of accepted errors)."@en ;
    dqv:expectedDataType xsd:boolean ;
    dqv:inDimension :DQ_ThematicClassificationCorrectness ;
    prov:wasDerivedFrom :D63.ISO.19157 .

:D68.ISO.19157_conformance a dqv:Metric ;
    skos:definition "Checks if the number of incorrect attribute values is below Ac (maximum number of accepted errors)."@en ;
    dqv:expectedDataType xsd:boolean ;
    dqv:inDimension :DQ_NonQuantitativeAttributeCorrectness ;
    prov:wasDerivedFrom :D68.ISO.19157 .

:DQ_DomainConsistency a dqv:Dimension ;
    skos:definition "Domain consistency refers to the degree of adherence of metadata element values to the value domains."@en ;
    skos:prefLabel "Domain consistency"@en ;
    dqv:inCategory :DQ_LogicalConsistency .

:OverallQualityOfFreeText_conformance a dqv:Metric ;
    skos:definition "Checks if the number of records using text values with a bad quality level is below Ac (maximum number of accepted errors)."@en ;
    dqv:expectedDataType xsd:boolean ;
    dqv:inDimension :DQ_QualityOfFreeText ;
    prov:wasDerivedFrom :OverallQualityOfFreeText .

:Sim_D33.ISO.19157_conformance a dqv:Metric ;
    skos:definition "Checks if the rate of records with positional errors (no overlapping between direct and indirect georeferences) is below AQL (statistical error level)."@en ;
    dqv:expectedDataType xsd:boolean ;
    dqv:inDimension :DQ_PositionalCorrectness ;
    prov:wasDerivedFrom :Sim_D33.ISO.19157 .

:onLanguage a qb:DimensionProperty,
        owl:DatatypeProperty ;
    rdfs:label "Label assessment language"@en ;
    rdfs:comment "Language on which the quality measure is assessed."@en ;
    rdfs:domain dqv:QualityMeasurement ;
    rdfs:range xsd:string .

:onProperty a qb:DimensionProperty,
        rdf:Property ;
    rdfs:label "Label assessment property"@en ;
    rdfs:comment "Property on which the quality measure is assessed."@en ;
    rdfs:domain dqv:QualityMeasurement ;
    rdfs:range rdf:Property .

:D.7.ISO.19157_conformance a dqv:Metric ;
    skos:definition "Checks if the rate of records with missing items is below AQL (statistical error level)."@en ;
    dqv:expectedDataType xsd:boolean ;
    dqv:inDimension :DQ_CompletenessOmission ;
    prov:wasDerivedFrom :D.7.ISO.19157 .

:D18.ISO.19157_conformance a dqv:Metric ;
    skos:definition "Checks if the value domain non-conformance rate is below AQL (statistical error level)."@en ;
    dqv:expectedDataType xsd:boolean ;
    dqv:inDimension :DQ_TemporalValidity ;
    prov:wasDerivedFrom :D18.ISO.19157 .

:D63.ISO.19157 a dqv:Metric ;
    skos:definition "Number of incorrectly classified records."@en ;
    dqv:expectedDataType xsd:integer ;
    dqv:inDimension :DQ_ThematicClassificationCorrectness .

:D68.ISO.19157 a dqv:Metric ;
    skos:definition "Number of incorrect attribute values."@en ;
    dqv:expectedDataType xsd:integer ;
    dqv:inDimension :DQ_NonQuantitativeAttributeCorrectness .

:D69.ISO.19157_conformance a dqv:Metric ;
    skos:definition "Checks if the rate of incorrect attribute values is below AQL (statistical error level)."@en ;
    dqv:expectedDataType xsd:boolean ;
    dqv:inDimension :DQ_NonQuantitativeAttributeCorrectness ;
    prov:wasDerivedFrom :D69.ISO.19157 .

:DQ_ComComDat_CR a dqv:QualityMeasurement ;
    dct:date "2022-05-11"^^xsd:date ;
    :onProperty dcat:dataset ;
    dqv:computedOn :myCatalog ;
    dqv:isMeasurementOf :D.3.ISO.19157_conformance ;
    dqv:value true ;
    prov:wasDerivedFrom :DQ_ComComDat_QR .

:DQ_ComComDis_CR a dqv:QualityMeasurement ;
    dct:date "2022-05-11"^^xsd:date ;
    :onProperty dcat:distribution ;
    dqv:computedOn :myCatalog ;
    dqv:isMeasurementOf :D.3.ISO.19157_conformance ;
    dqv:value true ;
    prov:wasDerivedFrom :DQ_ComComDis_QR .

:DQ_ComOmiDat_CR a dqv:QualityMeasurement ;
    dct:date "2022-05-11"^^xsd:date ;
    :onProperty dcat:dataset ;
    dqv:computedOn :myCatalog ;
    dqv:isMeasurementOf :D.7.ISO.19157_conformance ;
    dqv:value true ;
    prov:wasDerivedFrom :DQ_ComOmiDat_QR .

:DQ_ComOmiDis_CR a dqv:QualityMeasurement ;
    dct:date "2022-05-11"^^xsd:date ;
    :onProperty dcat:distribution ;
    dqv:computedOn :myCatalog ;
    dqv:isMeasurementOf :D.3.ISO.19157_conformance ;
    dqv:value false ;
    prov:wasDerivedFrom :DQ_ComOmiDis_QR .

:DQ_LogConDat_CR a dqv:QualityMeasurement ;
    dct:date "2022-05-11"^^xsd:date ;
    :onProperty dcat:dataset ;
    dqv:computedOn :myCatalog ;
    dqv:isMeasurementOf :D.13.ISO.19157_conformance ;
    dqv:value true ;
    prov:wasDerivedFrom :DQ_LogConDat_QR .

:DQ_LogConDis_CR a dqv:QualityMeasurement ;
    dct:date "2022-05-11"^^xsd:date ;
    :onProperty dcat:dataset ;
    dqv:computedOn :myCatalog ;
    dqv:isMeasurementOf :D.13.ISO.19157_conformance ;
    dqv:value false ;
    prov:wasDerivedFrom :DQ_LogConDis_QR .

:DQ_LogDomDatAcc_CR a dqv:QualityMeasurement ;
    dct:date "2022-05-11"^^xsd:date ;
    :onProperty dct:accrualPeriodicity,
        dcat:dataset ;
    dqv:computedOn :myCatalog ;
    dqv:isMeasurementOf :D.17.ISO.19157_conformance ;
    dqv:value true ;
    prov:wasDerivedFrom :DQ_LogDomDatAcc_QR .

:DQ_LogDomDatCon_CR a dqv:QualityMeasurement ;
    dct:date "2022-05-11"^^xsd:date ;
    :onProperty dct:conformsTo,
        dcat:dataset ;
    dqv:computedOn :myCatalog ;
    dqv:isMeasurementOf :D.17.ISO.19157_conformance ;
    dqv:value true ;
    prov:wasDerivedFrom :DQ_LogDomDatCon_QR .

:DQ_LogDomDatDes_CR a dqv:QualityMeasurement ;
    dct:date "2022-05-11"^^xsd:date ;
    :onProperty dct:description,
        dcat:dataset ;
    dqv:computedOn :myCatalog ;
    dqv:isMeasurementOf :D.17.ISO.19157_conformance ;
    dqv:value true ;
    prov:wasDerivedFrom :DQ_LogDomDatDes_QR .

:DQ_LogDomDatDis_CR a dqv:QualityMeasurement ;
    dct:date "2022-05-11"^^xsd:date ;
    :onProperty dcat:distribution ;
    dqv:computedOn :myCatalog ;
    dqv:isMeasurementOf :D.17.ISO.19157_conformance ;
    dqv:value true ;
    prov:wasDerivedFrom :DQ_LogDomDatDis_QR .

:DQ_LogDomDatIde_CR a dqv:QualityMeasurement ;
    dct:date "2022-05-11"^^xsd:date ;
    :onProperty dct:identifier,
        dcat:dataset ;
    dqv:computedOn :myCatalog ;
    dqv:isMeasurementOf :D.17.ISO.19157_conformance ;
    dqv:value true ;
    prov:wasDerivedFrom :DQ_LogDomDatIde_QR .

:DQ_LogDomDatIss_CR a dqv:QualityMeasurement ;
    dct:date "2022-05-11"^^xsd:date ;
    :onProperty dct:issued,
        dcat:dataset ;
    dqv:computedOn :myCatalog ;
    dqv:isMeasurementOf :D.17.ISO.19157_conformance ;
    dqv:value true ;
    prov:wasDerivedFrom :DQ_LogDomDatIss_QR .

:DQ_LogDomDatKey_CR a dqv:QualityMeasurement ;
    dct:date "2022-05-11"^^xsd:date ;
    :onProperty dcat:dataset,
        dcat:keyword ;
    dqv:computedOn :myCatalog ;
    dqv:isMeasurementOf :D.17.ISO.19157_conformance ;
    dqv:value true ;
    prov:wasDerivedFrom :DQ_LogDomDatKey_QR .

:DQ_LogDomDatLan_CR a dqv:QualityMeasurement ;
    dct:date "2022-05-11"^^xsd:date ;
    :onProperty dct:language,
        dcat:dataset ;
    dqv:computedOn :myCatalog ;
    dqv:isMeasurementOf :D.17.ISO.19157_conformance ;
    dqv:value true ;
    prov:wasDerivedFrom :DQ_LogDomDatLan_QR .

:DQ_LogDomDatMod_CR a dqv:QualityMeasurement ;
    dct:date "2022-05-11"^^xsd:date ;
    :onProperty dct:modified,
        dcat:dataset ;
    dqv:computedOn :myCatalog ;
    dqv:isMeasurementOf :D.17.ISO.19157_conformance ;
    dqv:value true ;
    prov:wasDerivedFrom :DQ_LogDomDatMod_QR .

:DQ_LogDomDatPub_CR a dqv:QualityMeasurement ;
    dct:date "2022-05-11"^^xsd:date ;
    :onProperty dct:publisher,
        dcat:dataset ;
    dqv:computedOn :myCatalog ;
    dqv:isMeasurementOf :D.17.ISO.19157_conformance ;
    dqv:value false ;
    prov:wasDerivedFrom :DQ_LogDomDatPub_QR .

:DQ_LogDomDatRef_CR a dqv:QualityMeasurement ;
    dct:date "2022-05-11"^^xsd:date ;
    :onProperty dct:references,
        dcat:dataset ;
    dqv:computedOn :myCatalog ;
    dqv:isMeasurementOf :D.17.ISO.19157_conformance ;
    dqv:value true ;
    prov:wasDerivedFrom :DQ_LogDomDatRef_QR .

:DQ_LogDomDatSpa_CR a dqv:QualityMeasurement ;
    dct:date "2022-05-11"^^xsd:date ;
    :onProperty dct:spatial,
        dcat:dataset ;
    dqv:computedOn :myCatalog ;
    dqv:isMeasurementOf :D.17.ISO.19157_conformance ;
    dqv:value false ;
    prov:wasDerivedFrom :DQ_LogDomDatSpa_QR .

:DQ_LogDomDatTem_CR a dqv:QualityMeasurement ;
    dct:date "2022-05-11"^^xsd:date ;
    :onProperty dct:temporal,
        dcat:dataset ;
    dqv:computedOn :myCatalog ;
    dqv:isMeasurementOf :D.17.ISO.19157_conformance ;
    dqv:value true ;
    prov:wasDerivedFrom :DQ_LogDomDatTem_QR .

:DQ_LogDomDatThe_CR a dqv:QualityMeasurement ;
    dct:date "2022-05-11"^^xsd:date ;
    :onProperty dcat:dataset,
        dcat:theme ;
    dqv:computedOn :myCatalog ;
    dqv:isMeasurementOf :D.17.ISO.19157_conformance ;
    dqv:value true ;
    prov:wasDerivedFrom :DQ_LogDomDatThe_QR .

:DQ_LogDomDatTit_CR a dqv:QualityMeasurement ;
    dct:date "2022-05-11"^^xsd:date ;
    :onProperty dct:title,
        dcat:dataset ;
    dqv:computedOn :myCatalog ;
    dqv:isMeasurementOf :D.17.ISO.19157_conformance ;
    dqv:value true ;
    prov:wasDerivedFrom :DQ_LogDomDatTit_QR .

:DQ_LogDomDatValid_CR a dqv:QualityMeasurement ;
    dct:date "2022-05-11"^^xsd:date ;
    :onProperty dct:valid,
        dcat:dataset ;
    dqv:computedOn :myCatalog ;
    dqv:isMeasurementOf :D.17.ISO.19157_conformance ;
    dqv:value true ;
    prov:wasDerivedFrom :DQ_LogDomDatValid_QR .

:DQ_LogDomDisByt_CR a dqv:QualityMeasurement ;
    dct:date "2022-05-11"^^xsd:date ;
    :onProperty dcat:byteSize,
        dcat:distribution ;
    dqv:computedOn :myCatalog ;
    dqv:isMeasurementOf :D.17.ISO.19157_conformance ;
    dqv:value true ;
    prov:wasDerivedFrom :DQ_LogDomDisByt_QR .

:DQ_LogDomDisFor_CR a dqv:QualityMeasurement ;
    dct:date "2022-05-11"^^xsd:date ;
    :onProperty dct:format,
        dcat:distribution ;
    dqv:computedOn :myCatalog ;
    dqv:isMeasurementOf :D.17.ISO.19157_conformance ;
    dqv:value false ;
    prov:wasDerivedFrom :DQ_LogDomDisFor_QR .

:DQ_LogDomDisIde_CR a dqv:QualityMeasurement ;
    dct:date "2022-05-11"^^xsd:date ;
    :onProperty dct:identifier,
        dcat:distribution ;
    dqv:computedOn :myCatalog ;
    dqv:isMeasurementOf :D.17.ISO.19157_conformance ;
    dqv:value true ;
    prov:wasDerivedFrom :DQ_LogDomDisIde_QR .

:DQ_LogDomDisTit_CR a dqv:QualityMeasurement ;
    dct:date "2022-05-11"^^xsd:date ;
    :onProperty dct:title,
        dcat:distribution ;
    dqv:computedOn :myCatalog ;
    dqv:isMeasurementOf :D.17.ISO.19157_conformance ;
    dqv:value true ;
    prov:wasDerivedFrom :DQ_LogDomDisTit_QR .

:DQ_PosCorrDatSpa_CR a dqv:QualityMeasurement ;
    dct:date "2022-05-11"^^xsd:date ;
    :onProperty dct:license,
        dcat:distribution ;
    dqv:computedOn :myCatalog ;
    dqv:isMeasurementOf :D69.ISO.19157_conformance ;
    dqv:value false ;
    prov:wasDerivedFrom :DQ_PosCorrDatSpa_QR .

:DQ_QFTDatDesR_CR a dqv:QualityMeasurement ;
    dct:date "2022-05-11"^^xsd:date ;
    :onProperty dct:title,
        dcat:dataset ;
    dqv:computedOn :myCatalog ;
    dqv:isMeasurementOf :ReadibilityOfTreeText_conformance ;
    dqv:value false ;
    prov:wasDerivedFrom :DQ_QFTDatDesR_QR .

:DQ_QFTDatTitR_CR a dqv:QualityMeasurement ;
    dct:date "2022-05-11"^^xsd:date ;
    :onProperty dct:title,
        dcat:dataset ;
    dqv:computedOn :myCatalog ;
    dqv:isMeasurementOf :ReadibilityOfTreeText_conformance ;
    dqv:value false ;
    prov:wasDerivedFrom :DQ_QFTDatTitR_QR .

:DQ_TemDatHar_CR a dqv:QualityMeasurement ;
    dct:date "2022-05-11"^^xsd:date ;
    :onProperty dct:issued,
        dct:modified,
        dct:valid,
        dcat:dataset ;
    dqv:computedOn :myCatalog ;
    dqv:isMeasurementOf :D18.ISO.19157_conformance ;
    dqv:value true ;
    prov:wasDerivedFrom :DQ_TemDatHar_QR .

:DQ_TemDatIss_CR a dqv:QualityMeasurement ;
    dct:date "2022-05-11"^^xsd:date ;
    :onProperty dct:issued,
        dct:modified,
        dct:valid,
        dcat:dataset ;
    dqv:computedOn :myCatalog ;
    dqv:isMeasurementOf :Sim_D.62.ISO.19157_conformance ;
    dqv:value false ;
    prov:wasDerivedFrom :DQ_TemDatIss_QR .

:OverallQualityOfFreeText a dqv:Metric ;
    skos:definition "Number of records using text values with a bad quality level."@en ;
    dqv:expectedDataType xsd:integer ;
    dqv:inDimension :DQ_QualityOfFreeText .

:Sim_D.62.ISO.19157_conformance a dqv:Metric ;
    skos:definition "Checks if the rate of records with conflict time sequences is below AQL (statistical error level)."@en ;
    dqv:expectedDataType xsd:boolean ;
    dqv:inDimension :DQ_TemporalConsistency ;
    prov:wasDerivedFrom :Sim_D.62.ISO.19157 .

:Sim_D33.ISO.19157 a dqv:Metric ;
    skos:definition "Rate of records with positional errors (no overlapping between direct and indirect georeferences)."@en ;
    dqv:expectedDataType xsd:double ;
    dqv:inDimension :DQ_PositionalCorrectness .

:D.13.ISO.19157_conformance a dqv:Metric ;
    skos:definition "Checks if the rate of records compliant with the conceptual schema is above 100 - AQL (statistical error level)."@en ;
    dqv:expectedDataType xsd:boolean ;
    dqv:inDimension :DQ_ConceptualConsistency ;
    prov:wasDerivedFrom :D.13.ISO.19157 .

:D18.ISO.19157 a dqv:Metric ;
    skos:definition "Value domain non-conformance rate."@en ;
    dqv:expectedDataType xsd:double ;
    dqv:inDimension :DQ_TemporalValidity .

:D69.ISO.19157 a dqv:Metric ;
    skos:definition "Rate of incorrect attribute values."@en ;
    dqv:expectedDataType xsd:double ;
    dqv:inDimension :DQ_NonQuantitativeAttributeCorrectness .

:DQ_ComComDat_QR a dqv:QualityMeasurement ;
    dct:date "2022-05-11"^^xsd:date ;
    :onProperty dcat:dataset ;
    dqv:computedOn :myCatalog ;
    dqv:isMeasurementOf :D.3.ISO.19157 ;
    dqv:value 1e+00 .

:DQ_ComComDis_QR a dqv:QualityMeasurement ;
    dct:date "2022-05-11"^^xsd:date ;
    :onProperty dcat:distribution ;
    dqv:computedOn :myCatalog ;
    dqv:isMeasurementOf :D.3.ISO.19157 ;
    dqv:value 1e+00 .

:DQ_ComOmiDat_QR a dqv:QualityMeasurement ;
    dct:date "2022-05-11"^^xsd:date ;
    :onProperty dcat:dataset ;
    dqv:computedOn :myCatalog ;
    dqv:isMeasurementOf :D.7.ISO.19157 ;
    dqv:value 9.999843e-01 .

:DQ_ComOmiDis_QR a dqv:QualityMeasurement ;
    dct:date "2022-05-11"^^xsd:date ;
    :onProperty dcat:distribution ;
    dqv:computedOn :myCatalog ;
    dqv:isMeasurementOf :D.7.ISO.19157 ;
    dqv:value 0e+00 .

:DQ_Completeness a dqv:Category ;
    skos:definition "Completeness refers to the degree in which the metadata elements are present or absent."@en ;
    skos:prefLabel "Completeness"@en .

:DQ_CompletenessCommission a dqv:Dimension ;
    skos:definition "Completeness commission refers to the degree in which there are excess instances of metadata elements in a metadata record."@en ;
    skos:prefLabel "Completeness commission"@en ;
    dqv:inCategory :DQ_Completeness .

:DQ_CompletenessOmission a dqv:Dimension ;
    skos:definition "Completeness ommission refers to the degree in which there are mandatory elements absent in metadata records."@en ;
    skos:prefLabel "Completeness ommission"@en ;
    dqv:inCategory :DQ_Completeness .

:DQ_LogConDat_QR a dqv:QualityMeasurement ;
    dct:date "2022-05-11"^^xsd:date ;
    :onProperty dcat:dataset ;
    dqv:computedOn :myCatalog ;
    dqv:isMeasurementOf :D.13.ISO.19157 ;
    dqv:value 1e+00 .

:DQ_LogConDis_QR a dqv:QualityMeasurement ;
    dct:date "2022-05-11"^^xsd:date ;
    :onProperty dcat:dataset ;
    dqv:computedOn :myCatalog ;
    dqv:isMeasurementOf :D.13.ISO.19157 ;
    dqv:value 0e+00 .

:DQ_LogDomDatAcc_QR a dqv:QualityMeasurement ;
    dct:date "2022-05-11"^^xsd:date ;
    :onProperty dct:accrualPeriodicity,
        dcat:dataset ;
    dqv:computedOn :myCatalog ;
    dqv:isMeasurementOf :D.17.ISO.19157 ;
    dqv:value 1e+00 .

:DQ_LogDomDatCon_QR a dqv:QualityMeasurement ;
    dct:date "2022-05-11"^^xsd:date ;
    :onProperty dct:conformsTo,
        dcat:dataset ;
    dqv:computedOn :myCatalog ;
    dqv:isMeasurementOf :D.17.ISO.19157 ;
    dqv:value 1e+00 .

:DQ_LogDomDatDes_QR a dqv:QualityMeasurement ;
    dct:date "2022-05-11"^^xsd:date ;
    :onProperty dct:description,
        dcat:dataset ;
    dqv:computedOn :myCatalog ;
    dqv:isMeasurementOf :D.17.ISO.19157 ;
    dqv:value 1e+00 .

:DQ_LogDomDatDis_QR a dqv:QualityMeasurement ;
    dct:date "2022-05-11"^^xsd:date ;
    :onProperty dcat:distribution ;
    dqv:computedOn :myCatalog ;
    dqv:isMeasurementOf :D.17.ISO.19157 ;
    dqv:value 1e+00 .

:DQ_LogDomDatIde_QR a dqv:QualityMeasurement ;
    dct:date "2022-05-11"^^xsd:date ;
    :onProperty dct:identifier,
        dcat:dataset ;
    dqv:computedOn :myCatalog ;
    dqv:isMeasurementOf :D.17.ISO.19157 ;
    dqv:value 9.999655e-01 .

:DQ_LogDomDatIss_QR a dqv:QualityMeasurement ;
    dct:date "2022-05-11"^^xsd:date ;
    :onProperty dct:issued,
        dcat:dataset ;
    dqv:computedOn :myCatalog ;
    dqv:isMeasurementOf :D.17.ISO.19157 ;
    dqv:value 1e+00 .

:DQ_LogDomDatKey_QR a dqv:QualityMeasurement ;
    dct:date "2022-05-11"^^xsd:date ;
    :onProperty dcat:dataset,
        dcat:keyword ;
    dqv:computedOn :myCatalog ;
    dqv:isMeasurementOf :D.17.ISO.19157 ;
    dqv:value 1e+00 .

:DQ_LogDomDatLan_QR a dqv:QualityMeasurement ;
    dct:date "2022-05-11"^^xsd:date ;
    :onProperty dct:language,
        dcat:dataset ;
    dqv:computedOn :myCatalog ;
    dqv:isMeasurementOf :D.17.ISO.19157 ;
    dqv:value 1e+00 .

:DQ_LogDomDatMod_QR a dqv:QualityMeasurement ;
    dct:date "2022-05-11"^^xsd:date ;
    :onProperty dct:modified,
        dcat:dataset ;
    dqv:computedOn :myCatalog ;
    dqv:isMeasurementOf :D.17.ISO.19157 ;
    dqv:value 1e+00 .

:DQ_LogDomDatPub_QR a dqv:QualityMeasurement ;
    dct:date "2022-05-11"^^xsd:date ;
    :onProperty dct:publisher,
        dcat:dataset ;
    dqv:computedOn :myCatalog ;
    dqv:isMeasurementOf :D.17.ISO.19157 ;
    dqv:value 0e+00 .

:DQ_LogDomDatRef_QR a dqv:QualityMeasurement ;
    dct:date "2022-05-11"^^xsd:date ;
    :onProperty dct:references,
        dcat:dataset ;
    dqv:computedOn :myCatalog ;
    dqv:isMeasurementOf :D.17.ISO.19157 ;
    dqv:value 9.999469e-01 .

:DQ_LogDomDatSpa_QR a dqv:QualityMeasurement ;
    dct:date "2022-05-11"^^xsd:date ;
    :onProperty dct:spatial,
        dcat:dataset ;
    dqv:computedOn :myCatalog ;
    dqv:isMeasurementOf :D.17.ISO.19157 ;
    dqv:value 7.222222e-01 .

:DQ_LogDomDatTem_QR a dqv:QualityMeasurement ;
    dct:date "2022-05-11"^^xsd:date ;
    :onProperty dct:temporal,
        dcat:dataset ;
    dqv:computedOn :myCatalog ;
    dqv:isMeasurementOf :D.17.ISO.19157 ;
    dqv:value 1e+00 .

:DQ_LogDomDatThe_QR a dqv:QualityMeasurement ;
    dct:date "2022-05-11"^^xsd:date ;
    :onProperty dcat:dataset,
        dcat:theme ;
    dqv:computedOn :myCatalog ;
    dqv:isMeasurementOf :D.17.ISO.19157 ;
    dqv:value 1e+00 .

:DQ_LogDomDatTit_QR a dqv:QualityMeasurement ;
    dct:date "2022-05-11"^^xsd:date ;
    :onProperty dct:title,
        dcat:dataset ;
    dqv:computedOn :myCatalog ;
    dqv:isMeasurementOf :D.17.ISO.19157 ;
    dqv:value 1e+00 .

:DQ_LogDomDatValid_QR a dqv:QualityMeasurement ;
    dct:date "2022-05-11"^^xsd:date ;
    :onProperty dct:valid,
        dcat:dataset ;
    dqv:computedOn :myCatalog ;
    dqv:isMeasurementOf :D.17.ISO.19157 ;
    dqv:value 1e+00 .

:DQ_LogDomDisByt_QR a dqv:QualityMeasurement ;
    dct:date "2022-05-11"^^xsd:date ;
    :onProperty dcat:byteSize,
        dcat:distribution ;
    dqv:computedOn :myCatalog ;
    dqv:isMeasurementOf :D.17.ISO.19157 ;
    dqv:value 9.857649e-01 .

:DQ_LogDomDisFor_QR a dqv:QualityMeasurement ;
    dct:date "2022-05-11"^^xsd:date ;
    :onProperty dct:format,
        dcat:distribution ;
    dqv:computedOn :myCatalog ;
    dqv:isMeasurementOf :D.17.ISO.19157 ;
    dqv:value 5.512821e-01 .

:DQ_LogDomDisIde_QR a dqv:QualityMeasurement ;
    dct:date "2022-05-11"^^xsd:date ;
    :onProperty dct:identifier,
        dcat:distribution ;
    dqv:computedOn :myCatalog ;
    dqv:isMeasurementOf :D.17.ISO.19157 ;
    dqv:value 1e+00 .

:DQ_LogDomDisTit_QR a dqv:QualityMeasurement ;
    dct:date "2022-05-11"^^xsd:date ;
    :onProperty dct:title,
        dcat:distribution ;
    dqv:computedOn :myCatalog ;
    dqv:isMeasurementOf :D.17.ISO.19157 ;
    dqv:value 1e+00 .

:DQ_LogicalConsistency a dqv:Category ;
    skos:definition "Logical consistency refers to the degree of adherence to logical rules of metadata structure."@en ;
    skos:prefLabel "Logical Consistency"@en .

:DQ_PosCorrDatSpa_QR a dqv:QualityMeasurement ;
    dct:date "2022-05-11"^^xsd:date ;
    :onProperty dct:license,
        dcat:distribution ;
    dqv:computedOn :myCatalog ;
    dqv:isMeasurementOf :D69.ISO.19157 ;
    dqv:value -1.56912e-05 .

:DQ_PositionalCorrectness a dqv:Category,
        dqv:Dimension ;
    skos:definition "Positional correctness refers to the degree of correctnes of metadata elements describing the geographic extent of a resource."@en ;
    skos:prefLabel "Positional correctness"@en .

:DQ_QFTDatDesR_QR a dqv:QualityMeasurement ;
    dct:date "2022-05-11"^^xsd:date ;
    :onLanguage "es" ;
    :onProperty dct:title,
        dcat:dataset ;
    dqv:computedOn :myCatalog ;
    dqv:isMeasurementOf :YAAAAAAAAA--ReadibilityOfTreeText ;
    dqv:value 6.044092e-01 .

:DQ_QFTDatTitR_QR a dqv:QualityMeasurement ;
    dct:date "2022-05-11"^^xsd:date ;
    :onLanguage "es" ;
    :onProperty dct:title,
        dcat:dataset ;
    dqv:computedOn :myCatalog ;
    dqv:isMeasurementOf :ReadibilityOfTreeText ;
    dqv:value 6.161619e-01 .

:DQ_TemDatHar_QR a dqv:QualityMeasurement ;
    dct:date "2022-05-11"^^xsd:date ;
    :onProperty dct:issued,
        dct:modified,
        dct:valid,
        dcat:dataset ;
    dqv:computedOn :myCatalog ;
    dqv:isMeasurementOf :D18.ISO.19157 ;
    dqv:value 9.955751e-01 .

:DQ_TemDatIss_QR a dqv:QualityMeasurement ;
    dct:date "2022-05-11"^^xsd:date ;
    :onProperty dct:issued,
        dct:modified,
        dct:valid,
        dcat:dataset ;
    dqv:computedOn :myCatalog ;
    dqv:isMeasurementOf :Sim_D.62.ISO.19157 ;
    dqv:value 8.910717e-01 .

:DQ_TemporalConsistency a dqv:Dimension ;
    skos:definition "Temporal consistency refers to the degree of correctness of ordered events or sequences, if reported, within a single metadata record."@en ;
    skos:prefLabel "Temporal consistency"@en ;
    dqv:inCategory :DQ_TemporalQuality .

:DQ_TemporalQuality a dqv:Category ;
    skos:definition "Temporal quality refers to the accuracy of the temporal metadata elements and temporal relationships of metadata elements."@en ;
    skos:prefLabel "Temporal quality"@en .

:DQ_TemporalValidity a dqv:Dimension ;
    skos:definition "Temporal consistency refers to the degree of validity of metadata time values with respect to a defined time range."@en ;
    skos:prefLabel "Temporal validity"@en ;
    dqv:inCategory :DQ_TemporalQuality .

:DQ_ThematicAccuracy a dqv:Category ;
    skos:definition "Thematic accuracy refers to the correctness of non-quantitative metadata elements and metadata elements related to classifications."@en ;
    skos:prefLabel "Thematic accuracy"@en .

:DQ_ThematicClassificationCorrectness a dqv:Dimension ;
    skos:definition "Thematic classification correctness refers to the degree of correctness of the thematic keywords and categories included in the metadata with respect to a universe of discourse."@en ;
    skos:prefLabel "Thematic classification correctness"@en ;
    dqv:inCategory :DQ_ThematicAccuracy .

:ReadibilityOfTreeText a dqv:Metric ;
    skos:definition "Rate of records using text values considered readable with a readability index (e.g. Flesch) above a threshold."@en ;
    dqv:expectedDataType xsd:double ;
    dqv:inDimension :DQ_QualityOfFreeText .

:ReadibilityOfTreeText_conformance a dqv:Metric ;
    skos:definition "Checks if the rate of records using text values considered readable with a readability index (e.g. Flesch) above a threshold is above 100 - AQL (statistical error level)."@en ;
    dqv:expectedDataType xsd:boolean ;
    dqv:inDimension :DQ_QualityOfFreeText ;
    prov:wasDerivedFrom :ReadibilityOfTreeText .

:Sim_D.62.ISO.19157 a dqv:Metric ;
    skos:definition "Rate of records with conflict time sequences."@en ;
    dqv:expectedDataType xsd:double ;
    dqv:inDimension :DQ_TemporalConsistency .

:D.13.ISO.19157 a dqv:Metric ;
    skos:definition "Rate of records compliant with the conceptual schema."@en ;
    dqv:expectedDataType xsd:double ;
    dqv:inDimension :DQ_ConceptualConsistency .

:D.3.ISO.19157 a dqv:Metric ;
    skos:definition "Rate of records with excess items."@en ;
    dqv:expectedDataType xsd:double ;
    dqv:inDimension :DQ_CompletenessCommission .

:D.3.ISO.19157_conformance a dqv:Metric ;
    skos:definition "Checks if the rate of records with excess items is below AQL (statistical error level)."@en ;
    dqv:expectedDataType xsd:boolean ;
    dqv:inDimension :DQ_CompletenessCommission ;
    prov:wasDerivedFrom :D.3.ISO.19157 .

:D.7.ISO.19157 a dqv:Metric ;
    skos:definition "Rate of records with missing items."@en ;
    dqv:expectedDataType xsd:double ;
    dqv:inDimension :DQ_CompletenessOmission .

:DQ_ConceptualConsistency a dqv:Dimension ;
    skos:definition "Conceptual consistency refers to the degree of adherence to the metadata schema."@en ;
    skos:prefLabel "Conceptual consistency"@en ;
    dqv:inCategory :DQ_LogicalConsistency .

:DQ_NonQuantitativeAttributeCorrectness a dqv:Dimension ;
    skos:definition "Non-quantitative attribute correctness refers to the degree of correctness of correctness of non-quantitative metadata elements in relation to a universe of discourse."@en ;
    skos:prefLabel "Non-quantitative attribute correctness"@en ;
    dqv:inCategory :DQ_ThematicAccuracy .

:DQ_QualityOfFreeText a dqv:Category,
        dqv:Dimension ;
    skos:definition "Quality of free text refers to the editorial quality in the content of free-text metadata elements."@en ;
    skos:prefLabel "Quality of free text"@en .

:D.17.ISO.19157_conformance a dqv:Metric ;
    skos:definition "Checks if the value domain conformance rate is above 100 - AQL (statistical error level)."@en ;
    dqv:expectedDataType xsd:boolean ;
    dqv:inDimension :DQ_ConceptualConsistency ;
    prov:wasDerivedFrom :D.17.ISO.19157 .

:D.17.ISO.19157 a dqv:Metric ;
    skos:definition "Value domain conformance rate."@en ;
    dqv:expectedDataType xsd:double ;
    dqv:inDimension :DQ_ConceptualConsistency .

:myCatalog a dcat:Catalog ;
    dct:title dqv:hasQualityMeasurement,
        "datos.gob.es" ;
    dqv:hasQualityMeasurement :DQ_ComComDat_CR,
        :DQ_ComComDat_QR,
        :DQ_ComComDis_CR,
        :DQ_ComComDis_QR,
        :DQ_ComOmiDat_CR,
        :DQ_ComOmiDat_QR,
        :DQ_ComOmiDis_CR,
        :DQ_ComOmiDis_QR,
        :DQ_LogConDat_CR,
        :DQ_LogConDat_QR,
        :DQ_LogConDis_CR,
        :DQ_LogConDis_QR,
        :DQ_LogDomDatAcc_CR,
        :DQ_LogDomDatAcc_QR,
        :DQ_LogDomDatCon_CR,
        :DQ_LogDomDatCon_QR,
        :DQ_LogDomDatDes_CR,
        :DQ_LogDomDatDes_QR,
        :DQ_LogDomDatDis_CR,
        :DQ_LogDomDatDis_QR,
        :DQ_LogDomDatIde_CR,
        :DQ_LogDomDatIde_QR,
        :DQ_LogDomDatIss_CR,
        :DQ_LogDomDatIss_QR,
        :DQ_LogDomDatKey_CR,
        :DQ_LogDomDatKey_QR,
        :DQ_LogDomDatLan_CR,
        :DQ_LogDomDatLan_QR,
        :DQ_LogDomDatMod_CR,
        :DQ_LogDomDatMod_QR,
        :DQ_LogDomDatPub_CR,
        :DQ_LogDomDatPub_QR,
        :DQ_LogDomDatRef_CR,
        :DQ_LogDomDatRef_QR,
        :DQ_LogDomDatSpa_CR,
        :DQ_LogDomDatSpa_QR,
        :DQ_LogDomDatTem_CR,
        :DQ_LogDomDatTem_QR,
        :DQ_LogDomDatThe_CR,
        :DQ_LogDomDatThe_QR,
        :DQ_LogDomDatTit_CR,
        :DQ_LogDomDatTit_QR,
        :DQ_LogDomDatValid_CR,
        :DQ_LogDomDatValid_QR,
        :DQ_LogDomDisByt_CR,
        :DQ_LogDomDisByt_QR,
        :DQ_LogDomDisFor_CR,
        :DQ_LogDomDisFor_QR,
        :DQ_LogDomDisIde_CR,
        :DQ_LogDomDisIde_QR,
        :DQ_LogDomDisTit_CR,
        :DQ_LogDomDisTit_QR,
        :DQ_PosCorrDatSpa_CR,
        :DQ_PosCorrDatSpa_QR,
        :DQ_QFTDatDesR_CR,
        :DQ_QFTDatDesR_QR,
        :DQ_QFTDatTitR_CR,
        :DQ_QFTDatTitR_QR,
        :DQ_TemDatHar_CR,
        :DQ_TemDatHar_QR,
        :DQ_TemDatIss_CR,
        :DQ_TemDatIss_QR .

