@prefix : <http://www.qualityreport.com/qr/>.
@prefix dcat:<http://www.w3.org/ns/dcat#>. 
@prefix dcterms:<http://purl.org/dc/terms/>.
@prefix xsd:<http://www.w3.org/2001/XMLSchema#>.
@prefix dqv:<http://www.w3.org/ns/dqv#>.
@prefix skos:<http://www.w3.org/2004/02/skos/core#>.
@prefix ldqd:<http://www.w3.org/2016/05/ldqd#> .
@prefix dct:<http://purl.org/dc/terms/>.
@prefix qb:<http://purl.org/linked-data/cube#>.
@prefix owl:<http://www.w3.org/2002/07/owl#>.
@prefix rdf:<http://www.w3.org/1999/02/22-rdf-syntax-ns#>.
@prefix rdfs:<http://www.w3.org/2000/01/rdf-schema#>.
@prefix prov: <http://www.w3.org/ns/prov#>.

#################################################################################
#### definition of categories, dimensions and metrics  ###
#################################################################################


##################################################################################
### Extra properties in the model

#Parameters of the measurements (derived from DQV specification)
:onLanguage
    a qb:DimensionProperty, owl:DatatypeProperty ;
    rdfs:comment   "Language on which the quality measure is assessed."@en ;
    rdfs:domain    dqv:QualityMeasurement;
    rdfs:label     "Label assessment language"@en ;
    rdfs:range       xsd:string.

:onProperty
    a qb:DimensionProperty, rdf:Property ;
    rdfs:comment 	"Property on which the quality measure is assessed."@en ;
    rdfs:domain 	dqv:QualityMeasurement ;
    rdfs:label  	"Label assessment property"@en ;
    rdfs:range     	rdf:Property.


#################################################################################
#### Completeness  ###

:DQ_Completeness a dqv:Category ;
    skos:prefLabel "Completeness"@en ;
    skos:definition "Completeness refers to the degree in which the metadata elements are present or absent."@en .

:DQ_CompletenessCommission a dqv:Dimension ;
    dqv:inCategory :DQ_Completeness ;
    skos:prefLabel "Completeness commission"@en ;
    skos:definition "Completeness commission refers to the degree in which there are excess instances of metadata elements in a metadata record."@en .

:D.3.ISO.19157 a dqv:Metric ;
    skos:definition "Rate of records with excess items."@en ;
    dqv:inDimension :DQ_CompletenessCommission ;
    dqv:expectedDataType xsd:double .

:D.3.ISO.19157_conformance a dqv:Metric ;
    prov:wasDerivedFrom :D.3.ISO.19157 ;
    skos:definition "Checks if the rate of records with excess items is below AQL (statistical error level)."@en ;
    dqv:inDimension :DQ_CompletenessCommission ;
    dqv:expectedDataType xsd:boolean .

:DQ_CompletenessOmission a dqv:Dimension ;
    dqv:inCategory :DQ_Completeness ;
    skos:prefLabel "Completeness ommission"@en ;
    skos:definition "Completeness ommission refers to the degree in which there are mandatory elements absent in metadata records."@en .

:D.7.ISO.19157 a dqv:Metric ;
    skos:definition "Rate of records with missing items."@en ;
    dqv:inDimension :DQ_CompletenessOmission;
    dqv:expectedDataType xsd:double .

:D.7.ISO.19157_conformance a dqv:Metric ;
    prov:wasDerivedFrom :D.7.ISO.19157 ;
    skos:definition "Checks if the rate of records with missing items is below AQL (statistical error level)."@en ;
    dqv:inDimension :DQ_CompletenessOmission;
    dqv:expectedDataType xsd:boolean .


##################################################################################
### Logical Consistency


:DQ_LogicalConsistency a dqv:Category ;
    skos:prefLabel "Logical Consistency"@en ;
    skos:definition "Logical consistency refers to the degree of adherence to logical rules of metadata structure."@en .

:DQ_ConceptualConsistency a dqv:Dimension ;
    dqv:inCategory :DQ_LogicalConsistency ;
    skos:prefLabel "Conceptual consistency"@en ;
    skos:definition "Conceptual consistency refers to the degree of adherence to the metadata schema."@en .

:D.13.ISO.19157 a dqv:Metric ;
    skos:definition "Rate of records compliant with the conceptual schema."@en ;
    dqv:inDimension :DQ_ConceptualConsistency ;
    dqv:expectedDataType xsd:double .

:D.13.ISO.19157_conformance a dqv:Metric ;
    prov:wasDerivedFrom :D.13.ISO.19157 ;
    skos:definition "Checks if the rate of records compliant with the conceptual schema is above 100 - AQL (statistical error level)."@en ;
    dqv:inDimension :DQ_ConceptualConsistency ;
    dqv:expectedDataType xsd:boolean .

:DQ_DomainConsistency a dqv:Dimension ;
    dqv:inCategory :DQ_LogicalConsistency ;
    skos:prefLabel "Domain consistency"@en ;
    skos:definition "Domain consistency refers to the degree of adherence of metadata element values to the value domains."@en .

:D.17.ISO.19157 a dqv:Metric ;
    skos:definition "Value domain conformance rate."@en ;
    dqv:inDimension :DQ_ConceptualConsistency ;
    dqv:expectedDataType xsd:double .

:D.17.ISO.19157_conformance a dqv:Metric ;
    prov:wasDerivedFrom :D.17.ISO.19157 ;
    skos:definition "Checks if the value domain conformance rate is above 100 - AQL (statistical error level)."@en ;
    dqv:inDimension :DQ_ConceptualConsistency ;
    dqv:expectedDataType xsd:boolean .



##################################################################################
### Temporal Accuracy


:DQ_TemporalQuality a dqv:Category ;
    skos:prefLabel "Temporal quality"@en ;
    skos:definition "Temporal quality refers to the accuracy of the temporal metadata elements and temporal relationships of metadata elements."@en .

:DQ_TemporalConsistency a dqv:Dimension ;
    dqv:inCategory :DQ_TemporalQuality ;
    skos:prefLabel "Temporal consistency"@en ;
    skos:definition "Temporal consistency refers to the degree of correctness of ordered events or sequences, if reported, within a single metadata record."@en .

:Sim_D.62.ISO.19157 a dqv:Metric ;
    skos:definition "Rate of records with conflict time sequences."@en ;
    dqv:inDimension :DQ_TemporalConsistency ;
    dqv:expectedDataType xsd:double .

:Sim_D.62.ISO.19157_conformance a dqv:Metric ;
    prov:wasDerivedFrom :Sim_D.62.ISO.19157 ;
    skos:definition "Checks if the rate of records with conflict time sequences is below AQL (statistical error level)."@en ;
    dqv:inDimension :DQ_TemporalConsistency ;
    dqv:expectedDataType xsd:boolean .

:DQ_TemporalValidity a dqv:Dimension ;
    dqv:inCategory :DQ_TemporalQuality ;
    skos:prefLabel "Temporal validity"@en ;
    skos:definition "Temporal consistency refers to the degree of validity of metadata time values with respect to a defined time range."@en .

:D18.ISO.19157 a dqv:Metric ;
    skos:definition "Value domain non-conformance rate."@en ;
    dqv:inDimension :DQ_TemporalValidity ;
    dqv:expectedDataType xsd:double .

:D18.ISO.19157_conformance a dqv:Metric ;
    prov:wasDerivedFrom :D18.ISO.19157 ;
    skos:definition "Checks if the value domain non-conformance rate is below AQL (statistical error level)."@en ;
    dqv:inDimension :DQ_TemporalValidity ;
    dqv:expectedDataType xsd:boolean .


##################################################################################
### Thematic Accuracy

:DQ_ThematicAccuracy a dqv:Category ;
    skos:prefLabel "Thematic accuracy"@en ;
    skos:definition "Thematic accuracy refers to the correctness of non-quantitative metadata elements and metadata elements related to classifications."@en .

:DQ_ThematicClassificationCorrectness a dqv:Dimension ;
    dqv:inCategory :DQ_ThematicAccuracy ;
    skos:prefLabel "Thematic classification correctness"@en ;
    skos:definition "Thematic classification correctness refers to the degree of correctness of the thematic keywords and categories included in the metadata with respect to a universe of discourse."@en .

:D63.ISO.19157 a dqv:Metric ;
    skos:definition "Number of incorrectly classified records."@en ;
    dqv:inDimension :DQ_ThematicClassificationCorrectness ;
    dqv:expectedDataType xsd:integer .

:D63.ISO.19157_conformance a dqv:Metric ;
    prov:wasDerivedFrom :D63.ISO.19157 ;
    skos:definition "Checks if the number of incorrectly classified records is below Ac (maximum number of accepted errors)."@en ;
    dqv:inDimension :DQ_ThematicClassificationCorrectness ;
    dqv:expectedDataType xsd:boolean .

:DQ_NonQuantitativeAttributeCorrectness a dqv:Dimension ;
    dqv:inCategory :DQ_ThematicAccuracy ;
    skos:prefLabel "Non-quantitative attribute correctness"@en ;
    skos:definition "Non-quantitative attribute correctness refers to the degree of correctness of correctness of non-quantitative metadata elements in relation to a universe of discourse."@en .

:D68.ISO.19157 a dqv:Metric ;
    skos:definition "Number of incorrect attribute values."@en ;
    dqv:inDimension :DQ_NonQuantitativeAttributeCorrectness ;
    dqv:expectedDataType xsd:integer .

:D68.ISO.19157_conformance a dqv:Metric ;
    prov:wasDerivedFrom :D68.ISO.19157 ;
    skos:definition "Checks if the number of incorrect attribute values is below Ac (maximum number of accepted errors)."@en ;
    dqv:inDimension :DQ_NonQuantitativeAttributeCorrectness ;
    dqv:expectedDataType xsd:boolean .

:D69.ISO.19157 a dqv:Metric ;
    skos:definition "Rate of incorrect attribute values."@en ;
    dqv:inDimension :DQ_NonQuantitativeAttributeCorrectness ;
    dqv:expectedDataType xsd:double .

:D69.ISO.19157_conformance a dqv:Metric ;
    prov:wasDerivedFrom :D69.ISO.19157 ;
    skos:definition "Checks if the rate of incorrect attribute values is below AQL (statistical error level)."@en ;
    dqv:inDimension :DQ_NonQuantitativeAttributeCorrectness ;
    dqv:expectedDataType xsd:boolean .




##################################################################################
### Positional Correctness

:DQ_PositionalCorrectness a dqv:Category, dqv:Dimension ;
    skos:prefLabel "Positional correctness"@en ;
    skos:definition "Positional correctness refers to the degree of correctnes of metadata elements describing the geographic extent of a resource."@en .

:Sim_D33.ISO.19157 a dqv:Metric ;
    skos:definition "Rate of records with positional errors (no overlapping between direct and indirect georeferences)."@en ;
    dqv:inDimension :DQ_PositionalCorrectness ;
    dqv:expectedDataType xsd:double .

:Sim_D33.ISO.19157_conformance a dqv:Metric ;
    prov:wasDerivedFrom :Sim_D33.ISO.19157 ;
    skos:definition "Checks if the rate of records with positional errors (no overlapping between direct and indirect georeferences) is below AQL (statistical error level)."@en ;
    dqv:inDimension :DQ_PositionalCorrectness ;
    dqv:expectedDataType xsd:boolean .




##################################################################################
### Quality of Free Text

:DQ_QualityOfFreeText a dqv:Category, dqv:Dimension ;
    skos:prefLabel "Quality of free text"@en ;
    skos:definition "Quality of free text refers to the editorial quality in the content of free-text metadata elements."@en .

:OverallQualityOfFreeText a dqv:Metric ;
    skos:definition "Number of records using text values with a bad quality level."@en ;
    dqv:inDimension :DQ_QualityOfFreeText ;
    dqv:expectedDataType xsd:integer .

:OverallQualityOfFreeText_conformance a dqv:Metric ;
    prov:wasDerivedFrom :OverallQualityOfFreeText ;
    skos:definition "Checks if the number of records using text values with a bad quality level is below Ac (maximum number of accepted errors)."@en ;
    dqv:inDimension :DQ_QualityOfFreeText ;
    dqv:expectedDataType xsd:boolean .

:ReadibilityOfTreeText a dqv:Metric ;
    skos:definition "Rate of records using text values considered readable with a readability index (e.g. Flesch) above a threshold."@en ;
    dqv:inDimension :DQ_QualityOfFreeText ;
    dqv:expectedDataType xsd:double .

:ReadibilityOfTreeText_conformance a dqv:Metric ;
    prov:wasDerivedFrom :ReadibilityOfTreeText ;
    skos:definition "Checks if the rate of records using text values considered readable with a readability index (e.g. Flesch) above a threshold is above 100 - AQL (statistical error level)."@en ;
    dqv:inDimension :DQ_QualityOfFreeText ;
    dqv:expectedDataType xsd:boolean .



#################################################################################
#### Quality Report  ###
#################################################################################

:myCatalog a dcat:Catalog ;
    dcterms:title
    dqv:hasQualityMeasurement  .