@prefix : <http://www.qualityreport.com/qr/>.
@prefix dcat:<http://www.w3.org/ns/dcat#>. 
@prefix dcterms:<http://purl.org/dc/terms/>.
@prefix xsd:<http://www.w3.org/2001/XMLSchema#>.
@prefix dqv:<http://www.w3.org/ns/dqv#>.
@prefix skos:<http://www.w3.org/2004/02/skos/core#>.
@prefix ldqd:<http://www.w3.org/2016/05/ldqd#> .
@prefix dct:<http://purl.org/dc/terms/>.
@prefix qb:<http://purl.org/linked-data/cube#>.
@prefix owl:<http://www.w3.org/2002/07/owl#>.
@prefix rdf:<http://www.w3.org/1999/02/22-rdf-syntax-ns#>.
@prefix rdfs:<http://www.w3.org/2000/01/rdf-schema#>.
@prefix prov: <http://www.w3.org/ns/prov#>.

#################################################################################
#### definition of categories, dimensions and metrics  ###
#################################################################################


##################################################################################
### Extra properties in the model

#Parameters of the measurements (derived from DQV specification)
:onLanguage
    a qb:DimensionProperty, owl:DatatypeProperty ;
    rdfs:comment   "Language on which the quality measure is assessed."@en ;
    rdfs:domain    dqv:QualityMeasurement;
    rdfs:label     "Label assessment language"@en ;
    rdfs:range       xsd:string.

:onProperty
    a qb:DimensionProperty, rdf:Property ;
    rdfs:comment 	"Property on which the quality measure is assessed."@en ;
    rdfs:domain 	dqv:QualityMeasurement ;
    rdfs:label  	"Label assessment property"@en ;
    rdfs:range     	rdf:Property.


#################################################################################
#### Findability  ###


:Findability a dqv:Category ;
    skos:prefLabel "Findability"@en ;
    skos:definition "Metrics that help people and machines in finding datasets."@en .

:KeywordAvailability a dqv:Dimension ;
    dqv:inCategory :Findability ;
    skos:prefLabel "Keyword usage"@en ;
    skos:definition "Keywords directly support the search and thus increase the findability of the data dataset."@en .

:KeywordAvailability_rate a dqv:Metric ;
    skos:definition "Rate metric: The system checks whether keywords are defined. The number of keywords has no impact to the score."@en ;
    dqv:inDimension :KeywordAvailability ;
    dqv:expectedDataType xsd:double .

:KeywordAvailability_points a dqv:Metric ;
    prov:wasDerivedFrom :CategoryAvailability ;
    skos:definition "Points metric (0-30): The system checks whether keywords are defined. The number of keywords has no impact to the score."@en ;
    dqv:inDimension :KeywordAvailability_rate ;
    dqv:expectedDataType xsd:double .

:CategoryAvailability a dqv:Dimension ;
    dqv:inCategory :Findability ;
    skos:prefLabel "Categories"@en ;
    skos:definition "Categories help users to explore datasets thematically."@en .

:CategoryAvailability_rate a dqv:Metric ;
    skos:definition "Rate metric: It is checked whether one or more categories are assigned to the dataset. The number of assigned categories has no impact to the score."@en ;
    dqv:inDimension :CategoryAvailability ;
    dqv:expectedDataType xsd:double .

:CategoryAvailability_points a dqv:Metric ;
    prov:wasDerivedFrom :CategoryAvailability ;
    skos:definition "Points metric (0-30): It is checked whether one or more categories are assigned to the dataset. The number of assigned categories has no impact to the score."@en ;
    dqv:inDimension :CategoryAvailability_rate ;
    dqv:expectedDataType xsd:double .

:SpatialAvailability a dqv:Dimension ;
    dqv:inCategory :Findability ;
    skos:prefLabel "Geo search"@en ;
    skos:definition "Usage of spatial information would enable users in order to find the dataset with a geo facetted search."@en .

:SpatialAvailability_rate a dqv:Metric ;
    skos:definition "Rate metric: It is checked wether the property is set or not."@en ;
    dqv:inDimension :SpatialAvailability ;
    dqv:expectedDataType xsd:double .

:SpatialAvailability_points a dqv:Metric ;
    prov:wasDerivedFrom :SpatialAvailability_rate ;
    skos:definition "Points metric (0-20): It is checked wether the property is set or not."@en ;
    dqv:inDimension :SpatialAvailability ;
    dqv:expectedDataType xsd:double .

:TemporalAvailability a dqv:Dimension ;
    dqv:inCategory :Findability ;
    skos:prefLabel "Time based search"@en ;
    skos:definition "Usage of temporal information would enable users for a timely based facetted search."@en .

:TemporalAvailability_rate a dqv:Metric ;
    skos:definition "Rate metric: It is checked wether the property is set or not."@en ;
    dqv:inDimension :TemporalAvailability ;
    dqv:expectedDataType xsd:double .

:TemporalAvailability_points a dqv:Metric ;
    prov:wasDerivedFrom :TemporalAvailability_rate ;
    skos:definition "Points metric (0-20): It is checked wether the property is set or not."@en ;
    dqv:inDimension :TemporalAvailability ;
    dqv:expectedDataType xsd:double .


##################################################################################
### Accessibility


:Accessibility a dqv:Category ;
    skos:prefLabel "Accessibility"@en ;
    skos:definition "Metrics used to determine whether access to the data referenced by the distributions is guaranteed."@en .

:AccessUrlStatusCode a dqv:Dimension ;
    dqv:inCategory :Accessibility ;
    skos:prefLabel "AccessURL accessibility"@en ;
    skos:definition "The AccessURL is not necessarily a direct link to the data, but also may refers to a URL that gives access to the dataset or where more information about the dataset is available."@en .

:AccessUrlStatusCode_rate a dqv:Metric ;
    skos:definition "Rate metric: The specified URL is checked for accessibility via a HTTP HEAD request. If the responded status code is in the 200 or 300 range, the accessibility of the resource is evaluated positively."@en ;
    dqv:inDimension :AccessUrlStatusCode ;
    dqv:expectedDataType xsd:double .

:AccessUrlStatusCode_points a dqv:Metric ;
    prov:wasDerivedFrom :AccessUrlStatusCode_rate ;
    skos:definition "Points metric (0-50): The specified URL is checked for accessibility via a HTTP HEAD request. If the responded status code is in the 200 or 300 range, the accessibility of the resource is evaluated positively."@en ;
    dqv:inDimension :AccessUrlStatusCode ;
    dqv:expectedDataType xsd:double .

:DownloadUrlAvailability a dqv:Dimension ;
    dqv:inCategory :Accessibility ;
    skos:prefLabel "DownloadURL"@en ;
    skos:definition "The downloadURL is a direct link to the referenced data."@en .

:DownloadUrlAvailability_rate a dqv:Metric ;
    skos:definition "Rate metric: It is checked wether the property is set or not."@en ;
    dqv:inDimension :DownloadUrlAvailability ;
    dqv:expectedDataType xsd:double .

:DownloadUrlAvailability_points a dqv:Metric ;
    prov:wasDerivedFrom :DownloadUrlAvailability_rate ;
    skos:definition "Points metric (0-20): It is checked wether the property is set or not."@en ;
    dqv:inDimension :DownloadUrlAvailability ;
    dqv:expectedDataType xsd:double .

:DownloadUrlStatusCode a dqv:Dimension ;
    dqv:inCategory :Accessibility ;
    skos:prefLabel "DownloadURL accessibility"@en ;
    skos:definition "The AccessURL is not necessarily a direct link to the data, but also may refers to a URL that gives access to the dataset or where more information about the dataset is available."@en .

:DownloadUrlStatusCode_rate a dqv:Metric ;
    skos:definition "Rate metric: The specified URL is checked for accessibility via a HTTP HEAD request. If the responded status code is in the 200 or 300 range, the accessibility of the resource is evaluated positively."@en ;
    dqv:inDimension :DownloadUrlStatusCode ;
    dqv:expectedDataType xsd:double .

:DownloadUrlStatusCode_points a dqv:Metric ;
    prov:wasDerivedFrom :DownloadUrlStatusCode_rate ;
    skos:definition "Points metric (0-30): The specified URL is checked for accessibility via a HTTP HEAD request. If the responded status code is in the 200 or 300 range, the accessibility of the resource is evaluated positively."@en ;
    dqv:inDimension :DownloadUrlStatusCode ;
    dqv:expectedDataType xsd:double .


##################################################################################
### Interoperability

:Interoperability a dqv:Category ;
    skos:prefLabel "Interoperability"@en ;
    skos:definition "Metrics used to determine whether a distribution is considered interoperable."@en .

:FormatAvailability a dqv:Dimension ;
    dqv:inCategory :Interoperability ;
    skos:prefLabel "Format"@en ;
    skos:definition "This field specifies the file format of the distribution."@en .

:FormatAvailability_rate a dqv:Metric ;
    skos:definition "Rate metric: It is checked wether the property is set or not."@en ;
    dqv:inDimension :FormatAvailability ;
    dqv:expectedDataType xsd:double .

:FormatAvailability_points a dqv:Metric ;
    prov:wasDerivedFrom :FormatAvailability_rate ;
    skos:definition "Points metric (0-20): It is checked wether the property is set or not."@en ;
    dqv:inDimension :FormatAvailability ;
    dqv:expectedDataType xsd:double .

:MediaTypeAvailability a dqv:Dimension ;
    dqv:inCategory :Interoperability ;
    skos:prefLabel "Media type"@en ;
    skos:definition "This field specifies the media type of the distribution."@en .

:MediaTypeAvailability_rate a dqv:Metric ;
    skos:definition "Rate metric: It is checked wether the property is set or not."@en ;
    dqv:inDimension :MediaTypeAvailability ;
    dqv:expectedDataType xsd:double .

:MediaTypeAvailability_points a dqv:Metric ;
    prov:wasDerivedFrom :FormatAvailability_rate ;
    skos:definition "Points metric (0-10): It is checked wether the property is set or not."@en ;
    dqv:inDimension :MediaTypeAvailability ;
    dqv:expectedDataType xsd:double .

:FormatMediaTypeVocabularyAlignment a dqv:Dimension ;
    dqv:inCategory :Interoperability ;
    skos:prefLabel "Format / Media type from vocabulary"@en ;
    skos:definition "Checks whether format and media type belong to a controlled vocabulary."@en .

:FormatMediaTypeVocabularyAlignment_rate a dqv:Metric ;
    skos:definition "Rate metric: The format vocabulary can be found in the data.europa.eu GitLab repository. The media type is check against the IANA list."@en ;
    dqv:inDimension :FormatAvailability ;
    dqv:expectedDataType xsd:double .

:FormatMediaTypeVocabularyAlignment_points a dqv:Metric ;
    prov:wasDerivedFrom :FormatAvailability_rate ;
    skos:definition "Points metric (0-10): The format vocabulary can be found in the data.europa.eu GitLab repository. The media type is check against the IANA list."@en ;
    dqv:inDimension :FormatAvailability ;
    dqv:expectedDataType xsd:double .

:FormatMediaTypeNonProprietary a dqv:Dimension ;
    dqv:inCategory :Interoperability ;
    skos:prefLabel "Non-proprietary"@en ;
    skos:definition "Checks if the format of the distribution is non-proprietary."@en .

:FormatMediaTypeNonProprietary_rate a dqv:Metric ;
    skos:definition "Rate metric: The distribution is considered as non-proprietary if the specified format is contained in the corresponding data.europa.eu GitLab repository vocabulary."@en ;
    dqv:inDimension :FormatMediaTypeNonProprietary ;
    dqv:expectedDataType xsd:double .

:FormatMediaTypeNonProprietary_points a dqv:Metric ;
    prov:wasDerivedFrom :FormatMediaTypeNonProprietary_rate ;
    skos:definition "Points metric (0-20): The distribution is considered as non-proprietary if the specified format is contained in the corresponding data.europa.eu GitLab repository vocabulary."@en ;
    dqv:inDimension :FormatMediaTypeNonProprietary ;
    dqv:expectedDataType xsd:double .

:FormatMediaTypeMachineInterpretable a dqv:Dimension ;
    dqv:inCategory :Interoperability ;
    skos:prefLabel "Format"@en ;
    skos:definition "Checks if the format of the distribution is machine-readable."@en .

:FormatMediaTypeMachineInterpretable_rate a dqv:Metric ;
    skos:definition "Rate metric: The distribution is considered as machine-readable if the specified format is contained in the corresponding data.europa.eu GitLab repository vocabulary."@en ;
    dqv:inDimension :FormatMediaTypeMachineInterpretable ;
    dqv:expectedDataType xsd:double .

:FormatMediaTypeMachineInterpretable_points a dqv:Metric ;
    prov:wasDerivedFrom :FormatMediaTypeMachineInterpretable_rate ;
    skos:definition "Points metric (0-20): The distribution is considered as machine-readable if the specified format is contained in the corresponding data.europa.eu GitLab repository vocabulary."@en ;
    dqv:inDimension :FormatMediaTypeMachineInterpretable ;
    dqv:expectedDataType xsd:double .

:DcatApCompliance a dqv:Dimension ;
    dqv:inCategory :Interoperability ;
    skos:prefLabel "DCAT-AP compliance"@en ;
    skos:definition "DCAT-AP compliance is calculated across all sources and datasets available on a catalogue. This check is only performed if the metadata is originally harvested as DCAT-AP or as a valid derivate. DCAT-AP is a specification for describing linked public data in Europe. The data.europa.eu portal may also harvest metadata which does not fully comply to DCAT-AP. In order to increase conformity to DCAT-AP, the MQA checks each metadata for its DCAT-AP compliance."@en .

:DcatApCompliance_rate a dqv:Metric ;
    skos:definition "Rate metric: The metadata is validated against a set of SHACL shapes. The metadata is not compliant, if the SHACL validation reports at least one issue. The MQA uses data.europa.eu's DCAT-AP SHACL validation service. SHACL is a recommendation from the W3C and is used for validating RDF graphs against a set of shapes."@en ;
    dqv:inDimension :DcatApCompliance ;
    dqv:expectedDataType xsd:double .

:DcatApCompliance_points a dqv:Metric ;
    prov:wasDerivedFrom :DcatApCompliance_rate ;
    skos:definition "Points metric (0-30): The metadata is validated against a set of SHACL shapes. The metadata is not compliant, if the SHACL validation reports at least one issue. The MQA uses data.europa.eu's DCAT-AP SHACL validation service. SHACL is a recommendation from the W3C and is used for validating RDF graphs against a set of shapes."@en ;
    dqv:inDimension :DcatApCompliance ;
    dqv:expectedDataType xsd:double .


##################################################################################
### Reusability

:Reusability a dqv:Category ;
    skos:prefLabel "Reusability"@en ;
    skos:definition "Metrics used to check the reusability of the data."@en .

:LicenceAvailability a dqv:Dimension ;
    dqv:inCategory :Reusability ;
    skos:prefLabel "License information"@en ;
    skos:definition "A license is valuable information for the reuse of data."@en .

:LicenceAvailability_rate a dqv:Metric ;
    skos:definition "Rate metric: It is checked wether the property is set or not."@en ;
    dqv:inDimension :LicenceAvailability ;
    dqv:expectedDataType xsd:double .

:LicenceAvailability_points a dqv:Metric ;
    prov:wasDerivedFrom :LicenceAvailability_rate ;
    skos:definition "Points metric (0-20): It is checked wether the property is set or not."@en ;
    dqv:inDimension :LicenceAvailability ;
    dqv:expectedDataType xsd:double .

:KnownLicence a dqv:Dimension ;
    dqv:inCategory :Reusability ;
    skos:prefLabel "License vocabulary"@en ;
    skos:definition "We would like to limit the indication of incorrect license information. For example, we encounter many CC licenses that lack versioning."@en .

:KnownLicence_rate a dqv:Metric ;
    skos:definition "Rate metric: The MQA recommends and credits the usage of controlled vocabularies. The data.europa.eu portal publishes its controlled vocabularies in GitLab. The vocabularies are derived from the EU Vocabularies."@en ;
    dqv:inDimension :KnownLicence ;
    dqv:expectedDataType xsd:double .

:KnownLicence_points a dqv:Metric ;
    prov:wasDerivedFrom :KnownLicence_rate ;
    skos:definition "Points metric (0-10): The MQA recommends and credits the usage of controlled vocabularies. The data.europa.eu portal publishes its controlled vocabularies in GitLab. The vocabularies are derived from the EU Vocabularies."@en ;
    dqv:inDimension :KnownLicence ;
    dqv:expectedDataType xsd:double .

:AccessRightsAvailability a dqv:Dimension ;
    dqv:inCategory :Reusability ;
    skos:prefLabel "Access restrictions"@en ;
    skos:definition "This field indicates whether the access to the data is public or restricted."@en .

:AccessRightsAvailability_rate a dqv:Metric ;
    skos:definition "Rate metric: It is checked wether the property is set or not."@en ;
    dqv:inDimension :AccessRightsAvailability ;
    dqv:expectedDataType xsd:double .

:AccessRightsAvailability_points a dqv:Metric ;
    prov:wasDerivedFrom :AccessRightsAvailability_rate ;
    skos:definition "Points metric (0-10): It is checked wether the property is set or not."@en ;
    dqv:inDimension :AccessRightsAvailability ;
    dqv:expectedDataType xsd:double .

:AccessRightsVocabularyAlignment a dqv:Dimension ;
    dqv:inCategory :Reusability ;
    skos:prefLabel "Access restrictions vocabulary"@en ;
    skos:definition "The use of a controlled vocabulary for access restrictions increases reusability."@en .

:AccessRightsVocabularyAlignment_rate a dqv:Metric ;
    skos:definition "Rate metric: It is checked whether the controlled vocabulary for access rights is used."@en ;
    dqv:inDimension :AccessRightsVocabularyAlignment ;
    dqv:expectedDataType xsd:double .

:AccessRightsVocabularyAlignment_points a dqv:Metric ;
    prov:wasDerivedFrom :AccessRightsVocabularyAlignment_rate ;
    skos:definition "Points metric (0-5): It is checked whether the controlled vocabulary for access rights is used."@en ;
    dqv:inDimension :AccessRightsVocabularyAlignment ;
    dqv:expectedDataType xsd:double .

:ContactPointAvailability a dqv:Dimension ;
    dqv:inCategory :Reusability ;
    skos:prefLabel "Contact point"@en ;
    skos:definition "The contact point contains inform whom to address in case of questions regarding the data."@en .

:ContactPointAvailability_rate a dqv:Metric ;
    skos:definition "Rate metric: It is checked wether the property is set or not."@en ;
    dqv:inDimension :ContactPointAvailability ;
    dqv:expectedDataType xsd:double .

:ContactPointAvailability_points a dqv:Metric ;
    prov:wasDerivedFrom :AccessRightsVocabularyAlignment_rate ;
    skos:definition "Points metric (0-20): It is checked wether the property is set or not."@en ;
    dqv:inDimension :ContactPointAvailability ;
    dqv:expectedDataType xsd:double .

:PublisherAvailability a dqv:Dimension ;
    dqv:inCategory :Reusability ;
    skos:prefLabel "Publisher"@en ;
    skos:definition "It is checked wether the Publisher is set or not."@en .

:PublisherAvailability_rate a dqv:Metric ;
    skos:definition "Rate metric: It is checked wether the property is set or not."@en ;
    dqv:inDimension :PublisherAvailability ;
    dqv:expectedDataType xsd:double .

:PublisherAvailability_points a dqv:Metric ;
    prov:wasDerivedFrom :AccessRightsVocabularyAlignment_rate ;
    skos:definition "Points metric (0-10): It is checked wether the property is set or not."@en ;
    dqv:inDimension :PublisherAvailability ;
    dqv:expectedDataType xsd:double .

##################################################################################
### Contextuality

:Contextuality a dqv:Category ;
    skos:prefLabel "Contextuality"@en ;
    skos:definition "Light weight properties, that provide more context to the user.."@en .

:RightsAvailability a dqv:Dimension ;
    dqv:inCategory :Contextuality ;
    skos:prefLabel "Rights"@en ;
    skos:definition "In some cases, a specific license cannot be applied to a dataset. The 'Rights' field can be used to specify a reference to a resource that will inform a user about the rights he has when using the dataset."@en .

:RightsAvailability_rate a dqv:Metric ;
    skos:definition "Rate metric: It is checked wether the property is set or not."@en ;
    dqv:inDimension :RightsAvailability ;
    dqv:expectedDataType xsd:double .

:RightsAvailability_points a dqv:Metric ;
    prov:wasDerivedFrom :RightsAvailability_rate ;
    skos:definition "Points metric (0-5): It is checked wether the property is set or not."@en ;
    dqv:inDimension :RightsAvailability ;
    dqv:expectedDataType xsd:double .

:ByteSizeAvailability a dqv:Dimension ;
    dqv:inCategory :Contextuality ;
    skos:prefLabel "File size"@en ;
    skos:definition "Specifies the size of the file in bytes."@en .

:ByteSizeAvailability_rate a dqv:Metric ;
    skos:definition "Rate metric: It is checked wether the property is set or not."@en ;
    dqv:inDimension :ByteSizeAvailability ;
    dqv:expectedDataType xsd:double .

:ByteSizeAvailability_points a dqv:Metric ;
    prov:wasDerivedFrom :ByteSizeAvailability_rate ;
    skos:definition "Points metric (0-5): It is checked wether the property is set or not."@en ;
    dqv:inDimension :ByteSizeAvailability ;
    dqv:expectedDataType xsd:double .

:DateIssuedAvailability a dqv:Dimension ;
    dqv:inCategory :Contextuality ;
    skos:prefLabel "Date of issue"@en ;
    skos:definition "The date on which the dataset or distribution was released."@en .

:DateIssuedAvailability_rate a dqv:Metric ;
    skos:definition "Rate metric: It is checked wether the property is set or not."@en ;
    dqv:inDimension :DateIssuedAvailability ;
    dqv:expectedDataType xsd:double .

:DateIssuedAvailability_points a dqv:Metric ;
    prov:wasDerivedFrom :DateIssuedAvailability_rate ;
    skos:definition "Points metric (0-5): It is checked wether the property is set or not."@en ;
    dqv:inDimension :DateIssuedAvailability ;
    dqv:expectedDataType xsd:double .

:DateModifiedAvailability a dqv:Dimension ;
    dqv:inCategory :Contextuality ;
    skos:prefLabel "Modification date"@en ;
    skos:definition "The date on which the dataset or distribution was last changed."@en .

:DateModifiedAvailability_rate a dqv:Metric ;
    skos:definition "Rate metric: It is checked wether the property is set or not."@en ;
    dqv:inDimension :DateModifiedAvailability ;
    dqv:expectedDataType xsd:double .

:DateModifiedAvailability_points a dqv:Metric ;
    prov:wasDerivedFrom :DateModifiedAvailability_rate ;
    skos:definition "Points metric (0-5): It is checked wether the property is set or not."@en ;
    dqv:inDimension :DateModifiedAvailability ;
    dqv:expectedDataType xsd:double .


#################################################################################
#### Quality Report  ###
#################################################################################

    :myCatalog a dcat:Catalog ;
        dcterms:title 
        dqv:hasQualityMeasurement  .

:myCatalog a dcat:Catalog ;
    dcterms:title "datos.gob.es" ;
    dqv:hasQualityMeasurement 
	:KeywordAvailability_rate_value,:KeywordAvailability_points_value,
	:CategoryAvailability_rate_value,:CategoryAvailability_points_value,
	:SpatialAvailability_rate_value,:SpatialAvailability_points_value,
	:TemporalAvailability_rate_value,:TemporalAvailability_points_value,
	:AccessUrlStatusCode_rate_value,:AccessUrlStatusCode_points_value,
	:DownloadUrlAvailability_rate_value,:DownloadUrlAvailability_points_value,
	:DownloadUrlStatusCode_rate_value,:DownloadUrlStatusCode_points_value,
	:FormatAvailability_rate_value,:FormatAvailability_points_value,
	:MediaTypeAvailability_rate_value,:MediaTypeAvailability_points_value,
	:FormatMediaTypeVocabularyAlignment_rate_value,:FormatMediaTypeVocabularyAlignment_points_value,
	:FormatMediaTypeNonProprietary_rate_value,:FormatMediaTypeNonProprietary_points_value,
	:FormatMediaTypeMachineInterpretable_rate_value,:FormatMediaTypeMachineInterpretable_points_value,
	:DcatApCompliance_rate_value,:DcatApCompliance_points_value,
	:LicenceAvailability_rate_value,:LicenceAvailability_points_value,
	:KnownLicence_rate_value,:KnownLicence_points_value,
	:AccessRightsAvailability_rate_value,:AccessRightsAvailability_points_value,
	:AccessRightsVocabularyAlignment_rate_value,:AccessRightsVocabularyAlignment_points_value,
	:ContactPointAvailability_rate_value,:ContactPointAvailability_points_value,
	:PublisherAvailability_rate_value,:PublisherAvailability_points_value,
	:RightsAvailability_rate_value,:RightsAvailability_points_value,
	:ByteSizeAvailability_rate_value,:ByteSizeAvailability_points_value,
	:DateIssuedAvailability_rate_value,:DateIssuedAvailability_points_value,
	:DateModifiedAvailability_rate_value,:DateModifiedAvailability_points_value.